modular now

Cache.v
@@ -18,22 +18,21 @@ Module Type DataTypes.
   Parameter time: Mesg -> Time.
   Parameter addr: Mesg -> Addr.
 
-  Parameter timestamp: Cache -> Addr -> Time -> Time.
+  Parameter timeStamp: Cache -> Addr -> Time -> Time.
   Parameter Channel: Type.
 
   Parameter mch rch: Channel.
 End DataTypes.
 
-Module Type Channel (dataTypes: DataTypes).
-  Import dataTypes.
+Module Type Channel (dt: DataTypes).
+  Import dt.
 
   Variable marksend: Channel -> Cache -> Cache -> Time -> Mesg -> Prop.
   Variable recv: Channel -> Cache -> Cache -> Time -> Mesg -> Prop.
 
-  Set Implicit Arguments.
   Section local.
-    Variable s: Channel.
-    Variable p c : Cache.
+    Context {s: Channel}.
+    Context {p c : Cache}.
     Axiom uniqMarksend1: forall {m n t}, marksend s p c t m -> marksend s p c t n -> m = n.
     Axiom uniqMarksend2: forall {m t1 t2}, marksend s p c t1 m -> marksend s p c t2 m -> t1 = t2.
     Axiom uniqRecv1: forall {m n t}, recv s p c t m -> recv s p c t n -> m = n.
@@ -42,8 +41,25 @@ Module Type Channel (dataTypes: DataTypes).
   End local.
 End Channel.
 
-Module ChnlPerAddr (dataTypes: DataTypes) (ch: Channel dataTypes).
-  Import dataTypes.
+Module Type ChannelPerAddr (dt: DataTypes).
+  Import dt.
+
+  Variable marksend: Channel -> Cache -> Cache -> Addr -> Time -> Mesg -> Prop.
+  Variable recv: Channel -> Cache -> Cache -> Addr -> Time -> Mesg -> Prop.
+
+  Section local.
+    Context {s: Channel}.
+    Context {p c : Cache} {a: Addr}.
+    Axiom uniqMarksend1: forall {m n t}, marksend s p c a t m -> marksend s p c a t n -> m = n.
+    Axiom uniqMarksend2: forall {m t1 t2}, marksend s p c a t1 m -> marksend s p c a t2 m -> t1 = t2.
+    Axiom uniqRecv1: forall {m n t}, recv s p c a t m -> recv s p c a t n -> m = n.
+    Axiom uniqRecv2: forall {m t1 t2}, recv s p c a t1 m -> recv s p c a t2 m -> t1 = t2.
+    Axiom recvImpMarkSend: forall {m t}, recv s p c a t m -> exists t', t' <= t /\ marksend s p c a t' m.
+  End local.
+End ChannelPerAddr.
+
+Module mkChannelPerAddr (dt: DataTypes) (ch: Channel dt) : ChannelPerAddr dt.
+  Import dt.
   Definition marksend ch p c a t m := ch.marksend ch p c t m /\ addr m = a.
   Definition recv ch p c a t m := ch.recv ch p c t m /\ addr m = a.
 
@@ -67,64 +83,64 @@ Module ChnlPerAddr (dataTypes: DataTypes) (ch: Channel dataTypes).
           t' <= t /\ marksend s p c a t' m) x (conj (proj1 Px) (conj (proj2 Px) (proj2 recvm)))
       end.
   End local.
-End ChnlPerAddr.
+End mkChannelPerAddr.
 
-Module Type System (dataTypes: DataTypes) (ch: Channel dataTypes).
-  Import dataTypes.
+Module Type LocalState (dt: DataTypes).
+  Import dt.
+  Parameter st: Addr -> Time -> State.
+  Parameter src dst: Cache.
+  Parameter toRSComp: State -> State -> Prop.
+End LocalState.
 
-  Axiom classical: forall P, P \/ ~ P.
+Module Type LocalBehavior (dt: DataTypes) (ch: ChannelPerAddr dt).
+  Import dt ch.
 
-  Definition toCompat s := 3 - s.
+  Parameter st: Addr -> Time -> State.
+  Parameter src dst: Cache.
+  Parameter toRSComp: State -> State -> Prop.
 
-  Definition compat c p (rel: parent c = p) t := forall c', parent c' = p ->
-    forall a, dir p c' a t <= toCompat (dir p c a t).
+  Section ForT.
+    Context {t: Time}.
+    Context {a: Addr}.
 
-  Module Type LocalState.
-    Parameter st : Addr -> Time -> State.
-    Parameter mmarksend: Addr -> Time -> Mesg -> Prop.
-    Parameter mrecv: Addr -> Time -> Mesg -> Prop.
-    Parameter rmarksend: Addr -> Time -> Mesg -> Prop.
-    Parameter rrecv: Addr -> Time -> Mesg -> Prop.
-    Parameter toRSComp: State -> State -> Prop.
-    Parameter timeStamp: Addr -> Time -> Time.
-  End LocalState.
+    Axiom change: st a (S t) <> st a t -> (exists m, marksend mch src dst a t m) \/
+      (exists m, recv mch dst src a t m).
+    Axiom sendmChange: forall {m}, marksend mch src dst a t m -> st a (S t) = to m.
+    Axiom recvmChange: forall {m}, recv mch dst src a t m -> st a (S t) = to m.
+    Axiom sendrImpSt: forall {r}, marksend rch src dst a t r -> toRSComp (to r) (st a t).
+    Axiom sendrImpNoSendr: forall {t1 t2 r1 r2}, t1 < t2 -> marksend rch src dst a t1 r1 ->
+      marksend rch src dst a t2 r2 -> exists t', t1 < t' <= t2 /\ ~ toRSComp (to r1) (st a t').
+    Axiom sendmFrom: forall {m}, marksend mch src dst a t m -> from m = st a t.
+    Axiom sendrFrom: forall {r}, marksend rch src dst a t r -> from r = st a t.
+    Axiom sendmTime: forall {m}, marksend mch src dst a t m -> time m = timeStamp src a t.
+    Axiom noSendmRecvm: forall {m}, marksend mch src dst a t m ->
+      forall {m'}, recv mch dst src a t m' -> False.
+    Axiom noSendmSendr: forall {m}, marksend mch src dst a t m -> forall {r}, marksend rch src dst a t r -> False.
+  End ForT.
+End LocalBehavior.
 
-  Module StateBehave (s : LocalState).
-    Import s.
+Module LocalLemmas (dt: DataTypes) (ch: ChannelPerAddr dt) (lb: LocalBehavior dt ch).
+  Import dt lb ch.
 
-    Set Implicit Arguments.
-    Section ForT.
-      Variable t: Time.
-      Variable a: Addr.
-      Axiom change: st a (S t) <> st a t -> (exists m, mmarksend a t m) \/ (exists m, mrecv a t m).
-      Axiom sendmChange: forall {m}, mmarksend a t m -> st a (S t) = to m.
-      Axiom recvmChange: forall {m}, mrecv a t m -> st a (S t) = to m.
-      Axiom sendrImpSt: forall {r}, rmarksend a t r -> toRSComp (to r) (st a t).
-      Axiom sendrImpNoSendr: forall {t1 t2 r1 r2}, t1 < t2 -> rmarksend a t1 r1 -> rmarksend a t2 r2 ->
-        exists t', t1 < t' <= t2 /\ ~ toRSComp (to r1) (st a t').
-      Axiom sendmFrom: forall {m}, mmarksend a t m -> from m = st a t.
-      Axiom sendrFrom: forall {r}, rmarksend a t r -> from r = st a t.
-      Axiom sendmTime: forall {m}, mmarksend a t m -> time m = timeStamp a t.
-      Axiom noSendmRecvm: forall {m}, mmarksend a t m -> forall {m'}, mrecv a t m' -> False.
-      Axiom noSendmSendr: forall {m}, mmarksend a t m -> forall {r}, rmarksend a t r -> False.
-    End ForT.
-
+  Section ForLs.
     Lemma nochange': forall {a t t'}, (forall tn, t <= tn < t + t' ->
-      (forall m, ~ mmarksend a tn m) /\ (forall m, ~ mrecv a tn m)) -> st a t = st a (t + t').
+      (forall m, ~ marksend mch src dst a tn m) /\ (forall m, ~ recv mch dst src a tn m)) ->
+    st a t = st a (t + t').
     Proof.
       intros a t t'.
       induction t'.
       intro false.
       firstorder.
       intros noChange.
-      assert (help: forall tn, t <= tn < t + t' -> (forall m, ~ mmarksend a tn m) /\
-        (forall m, ~ mrecv a tn m)) by (
-        intros tn comp;
-          assert (comp2: t <= tn < t + S t') by omega;
-            firstorder).
+      assert (help: forall tn, t <= tn < t + t' -> (forall m, ~ marksend mch src dst a tn m) /\
+        (forall m, ~ recv mch dst src a tn m)) by (
+          intros tn comp;
+            assert (comp2: t <= tn < t + S t') by omega;
+              firstorder).
       assert (stTEqstT': st a t = st a (t + t')) by firstorder.
-      assert (nothing: (forall m, ~ mmarksend a (t + t') m) /\ forall m, ~ mrecv a (t + t') m) by
-        (assert (t <= t + t' < t + S t'); firstorder).
+      assert (nothing: (forall m, ~ marksend mch src dst a (t + t') m) /\
+        forall m, ~ recv mch dst src a (t + t') m) by
+      (assert (t <= t + t' < t + S t'); firstorder).
       rewrite stTEqstT'.
       assert (two: st a (t + S t') = st a (t + t') \/ st a (t + S t') <> st a (t + t')) by decide equality.
       destruct two as [easy | hard].
@@ -136,7 +152,7 @@ Module Type System (dataTypes: DataTypes) (ch: Channel dataTypes).
     Qed.
 
     Lemma noChange: forall {a t t'}, t < t' -> (forall tn, t <= tn < t' ->
-      (forall m, ~ mmarksend a tn m) /\ (forall m, ~ mrecv a tn m)) -> st a t = st a t'.
+      (forall m, ~ marksend mch src dst a tn m) /\ (forall m, ~ recv mch dst src a tn m)) -> st a t = st a t'.
     Proof.
       intros a t t' tLtT'.
       remember (t' - t) as td.
@@ -146,7 +162,7 @@ Module Type System (dataTypes: DataTypes) (ch: Channel dataTypes).
     Qed.
 
     Lemma noChange2: forall {a t t'}, t <= t' -> (forall tn, t <= tn < t' ->
-      (forall m, ~ mmarksend a tn m) /\ (forall m, ~ mrecv a tn m)) -> st a t = st a t'.
+      (forall m, ~ marksend mch src dst a tn m) /\ (forall m, ~ recv mch dst src a tn m)) -> st a t = st a t'.
     Proof.
       intros a t t' tLeT'.
       assert (opts: t = t' \/ t < t') by omega.
@@ -155,172 +171,77 @@ Module Type System (dataTypes: DataTypes) (ch: Channel dataTypes).
       reflexivity.
       apply noChange; intuition.
     Qed.
-  End StateBehave.
+  End ForLs.
+End LocalLemmas.
 
-  Module Type LocalRules.
-    Module chPerA := ChnlPerAddr dataTypes ch.
-    Import chPerA.
+Module Type Pair (dt: DataTypes).
+  Variable p c : dt.Cache.
+  Variable isParent : dt.parent c = p.
+End Pair.
 
-    Variables p c: Cache.
-    Hypothesis rel: parent c = p.
+Module Type StSemi (dt: DataTypes) (p: Pair dt) (ch: ChannelPerAddr dt) :=
+  LocalBehavior dt ch with
+  Definition st := dt.state p.c with
+    Definition src := p.c with
+      Definition dst := p.p with
+        Definition toRSComp := gt.
 
-    Module Dir <: LocalState.
-      Section ForT.
-        Variable a: Addr.
-        Variable t: Time.
+Module Type DirSemi (dt: DataTypes) (p: Pair dt) (ch: ChannelPerAddr dt) :=
+  LocalBehavior dt ch with
+  Definition st := dt.dir p.p p.c with
+    Definition src := p.p with
+      Definition dst := p.c with
+        Definition toRSComp := lt.
 
-        Definition st := dir p c.
-        Definition mmarksend := marksend mch p c.
-        Definition mrecv := recv mch c p.
-        Definition rmarksend := marksend rch p c.
-        Definition rrecv := recv rch c p.
-        Definition toRSComp x y := x < y.
-        Definition timeStamp := timestamp p.
-      End ForT.
-    End Dir.
+Module Type StBase (dt: DataTypes) (p: Pair dt) (ch: ChannelPerAddr dt) (st: StSemi dt p ch).
+  Module ll := LocalLemmas dt ch st.
+  Include ll.
+  Include st.
+  Import dt p ch.
 
-    Module St <: LocalState.
-      Section ForT.
-        Variable a: Addr.
-        Variable t: Time.
+  Section ForT.
+    Context {a: Addr} {t: Time}.
 
-        Definition st := state c.
-        Definition mmarksend := marksend mch c p.
-        Definition mrecv := recv mch p c.
-        Definition rmarksend := marksend rch c p.
-        Definition rrecv := recv rch p c.
-        Definition toRSComp x y := x > y.
-        Definition timeStamp := timestamp c.
+    Axiom sendmImpSt: forall {m}, marksend mch c p a t m -> state c a t > to m.
 
-      End ForT.
-    End St.
+    Axiom voluntary:
+      forall {r}, marksend rch c p a t r -> forall {t' m}, t' > t -> marksend mch c p a t' m ->
+        (forall {tm}, t < tm <= t' -> state c a tm < to r) -> exists r1, recv rch p c a t' r1.
 
-    Module db := StateBehave Dir.
+    Axiom recvrNoSendm: forall {r}, recv rch p c a t r -> forall {m}, marksend mch c p a t m ->
+      state c a t > to r.
 
-    Module sb := StateBehave St.
+    Axiom recvrSendm: forall {r}, recv rch p c a t r -> state c a t > to r -> exists {m}, marksend mch c p a t m.
+  End ForT.
+End StBase.
 
-    Set Implicit Arguments.
-    Definition twoEqPRespFalse := forall a t t1 m1, t1 <= t -> marksend mch p c a t1 m1 ->
-      forall t2 m2, t2 <= t -> marksend mch p c a t2 m2 ->
-        (forall t3, t3 <= t -> ~ recv mch p c a t3 m1) -> (forall {t4}, t4 <= t -> ~ recv mch p c a t4 m2) ->
-        t1 = t2.
+Module St (dt: DataTypes) (p: Pair dt) (ch: ChannelPerAddr dt) (st: StSemi dt p ch) (base: StBase dt p ch st).
+  Include base.
+  Import dt ch st p base.
 
-    Definition twoPReqNeedsResp := forall a t t1 r1, t1 <= t -> marksend rch p c a t1 r1 -> forall t2 r2,
-      t2 <= t -> marksend rch p c a t2 r2 -> (forall t3, t3 <= t -> ~ recv rch p c a t3 r1) ->
-      (forall t4, t4 <= t -> ~ recv rch p c a t4 r2) -> to r1 = to r2 -> t1 < t2 ->
-      exists tm m, t1 < tm < t2 /\ marksend mch p c a tm m.
-
-    Section ForT.
-      Variable a: Addr.
-      Variable t: Time.
-
-      Axiom init: dir p c a 0 = state c a 0.
-
-      Axiom stSendmImpSt: forall {m}, marksend mch c p a t m -> state c a t > to m.
-
-      Axiom dirSendmImpRecvr: forall {m}, marksend mch p c a t m -> exists r, recv rch c p a t r.
-
-      Axiom dirSendmImpRecvrGe: forall {m}, marksend mch p c a t m -> forall {r}, recv rch c p a t r -> to m >= to r.
-
-      Axiom dirRecvrCond: forall {r}, recv rch c p a t r -> from r >= dir p c a t.
-
-      Axiom dirRecvmCond: forall {m}, recv mch c p a t m -> from m = dir p c a t.
-
-      Axiom pRespReq: twoEqPRespFalse -> twoPReqNeedsResp -> forall {t1 t2 t3},
-        forall {m}, marksend mch p c a t1 m ->
-        forall {r}, marksend rch p c a t2 r -> recv rch p c a t3 r -> t1 <= t2 ->
-          exists t4, t4 < t3 /\ recv mch p c a t4 m.
-
-      Axiom pReqResp: twoEqPRespFalse -> twoPReqNeedsResp -> forall {t1 t2 t3},
-        forall {r}, marksend rch p c a t1 r ->
-        forall {m}, marksend mch p c a t2 m -> recv mch p c a t3 m -> t1 <= t2 ->
-          exists t4, t4 < t3 /\ recv rch p c a t4 r.
-
-      Axiom stVoluntary:
-        forall {r}, marksend rch c p a t r -> forall {t' m}, t' > t -> marksend mch c p a t' m ->
-          (forall {tm}, t < tm <= t' -> state c a tm < to r) -> exists r1, recv rch p c a t' r1.
-
-      Axiom dirSendrImpNoSendm: forall {t1 t2 r1 m2}, t1 < t2 -> marksend rch p c a t1 r1 ->
-        marksend mch p c a t2 m2 ->
-        exists t', t1 < t' < t2 /\ exists m, recv mch c p a t' m /\ to m <= to r1.
-
-      Axiom stRecvrNoSendm: forall {r}, recv rch p c a t r -> forall {m}, marksend mch c p a t m ->
-        state c a t > to r.
-
-      Axiom stRecvrSendm: forall {r}, recv rch p c a t r -> state c a t > to r -> exists {m}, marksend mch c p a t m.
-
-      Lemma whenChildHighRecvm: state c a (S t) > state c a t -> exists m,
-        recv mch p c a t m /\ to m = state c a (S t).
-      Proof.
-        intro sStgst.
-        assert (sStnst: state c a (S t) <> state c a t) by omega.
-        pose proof (sb.change sStnst) as [[m sendmm] | [m recvmm] ].
-        pose proof (stSendmImpSt sendmm) as stgm.
-        pose proof (sb.sendmChange sendmm) as sStem.
-        unfold St.mmarksend in *.
-        unfold St.st in *.
-        omega.
-        exists m.
-        intuition.
-        pose proof (sb.recvmChange recvmm) as sStem.
-        unfold St.mrecv in *.
-        unfold St.st in *.
-        intuition.
-      Qed.
-    End ForT.
-
-    Lemma dirRecvImpLow: forall {a t m}, recv mch c p a t m -> dir p c a t > dir p c a (S t).
+  Section ForT.
+    Context {a: Addr}.
+    Lemma whenChildHighRecvm: forall {t}, state c a (S t) > state c a t -> exists m,
+      recv mch p c a t m /\ to m = state c a (S t).
     Proof.
-      intros a t m recvm.
-      pose proof (recvImpMarkSend recvm) as [t' [t'LeT sendm]].
-      pose proof (db.recvmChange recvm) as sth.
-      pose proof (stSendmImpSt sendm) as sth2.
-      pose proof (dirRecvmCond recvm) as sth3.
-      pose proof (sb.sendmFrom sendm) as sth4.
-      unfold Dir.st, St.st in *.
+      intros t sStgst.
+      assert (sStnst: state c a (S t) <> state c a t) by omega.
+      pose proof (change sStnst) as [[m sendmm] | [m recvmm] ].
+      pose proof (sendmImpSt sendmm) as stgm.
+      pose proof (sendmChange sendmm) as sStem.
+      unfold st in *.
       omega.
+      exists m.
+      intuition.
+      pose proof (recvmChange recvmm) as sStem.
+      unfold src, dst in *.
+      intuition.
     Qed.
 
-    Lemma whenDirLow': forall {a t t'}, dir p c a (t' + t) > dir p c a t ->
-      exists t'', t'' < t' /\ exists m, marksend mch p c a (t'' + t) m.
-    Proof.
-      intros a t t'.
-      induction t'.
-      intros dirGt.
-      unfold plus in *; simpl. omega.
-      intros dirGt.
-      assert (opts: dir p c a (t' + t) > dir p c a t \/ dir p c a (t' + t) <= dir p c a t) by omega.
-      destruct opts as [gt | le].
-      firstorder.
-      assert (gt: dir p c a (S (t' + t)) > dir p c a (t' + t)) by (assert (eq: S t' + t = S (t' + t)) by omega;
-        rewrite eq in *; omega).
-      assert (nestuff: dir p c a (S (t' + t)) <> dir p c a (t' + t)) by omega.
-      pose proof (db.change nestuff) as [sendm | recvm].
-      firstorder.
-      destruct recvm as [x recvstuff].
-      pose proof (dirRecvImpLow recvstuff) as contra.
-      omega.
-    Qed.
-
-    Lemma whenDirLow: forall {a t t1}, t <= t1 -> dir p c a t1 > dir p c a t ->
-      exists t'', t <= t'' < t1 /\ exists m, marksend mch p c a t'' m.
-    Proof.
-      intros a t t1 t1LeT1 dirGt.
-      assert (opt: t = t1 \/ t < t1) by omega.
-      destruct opt as [tEqT1 | tLeT1].
-      rewrite tEqT1 in *; omega.
-      remember (t1 - t - 1) as t'.
-      assert (eq: t1 = (t' + 1) + t) by omega.
-      rewrite eq in *.
-      pose proof (whenDirLow' dirGt) as [t'' [t''Cond ext]]. 
-      exists (t'' + t).
-      firstorder.
-    Qed.
-
-    Lemma whenChildHigh': forall {a t t'}, state c a (S (t' + t)) > state c a t ->
+    Lemma whenChildHigh': forall {t t'}, state c a (S (t' + t)) > state c a t ->
       exists t'', t'' <= t' /\ exists m, recv mch p c a (t'' + t) m /\ to m >= state c a (S (t' + t)).
     Proof.
-      intros a t t' sSt'tgst.
+      intros t t' sSt'tgst.
       induction t'.
       pose proof (whenChildHighRecvm sSt'tgst) as [m [recvmm mesSt]].
       exists 0.
@@ -352,10 +273,10 @@ Module Type System (dataTypes: DataTypes) (ch: Channel dataTypes).
       intuition.
     Qed.
 
-    Lemma whenChildHigh: forall {a t t'}, t' > t -> state c a t' > state c a t ->
+    Lemma whenChildHigh: forall {t t'}, t' > t -> state c a t' > state c a t ->
       exists t'', t <= t'' < t' /\ exists m, recv mch p c a t'' m /\ to m >= state c a t'.
     Proof.
-      intros a t tPlust'.
+      intros t tPlust'.
       intros diff.
       remember (tPlust' - S t) as t'.
       assert (eq: tPlust' = S (t' + t)) by omega.
@@ -368,11 +289,11 @@ Module Type System (dataTypes: DataTypes) (ch: Channel dataTypes).
       assumption.
     Qed.
 
-    Lemma whenChildHighConv: forall {a t t'}, t' >= t ->
+    Lemma whenChildHighConv: forall {t t'}, t' >= t ->
       (~ exists t'', t <= t'' < t' /\ exists m, recv mch p c a t'' m /\ to m >= state c a t') ->
       state c a t' <= state c a t.
     Proof.
-      intros a t t' t'GeT notE.
+      intros t t' t'GeT notE.
       assert (opts: t' = t \/ t' > t) by omega.
       destruct opts as [t'EqT | t'GtT].
       rewrite t'EqT; reflexivity.
@@ -380,327 +301,461 @@ Module Type System (dataTypes: DataTypes) (ch: Channel dataTypes).
         pose proof (whenChildHigh t'GtT one); firstorder).
       omega.
     Qed.
+  End ForT.
+End St.
 
-    Lemma cReqPRespCrossInd: forall {a t tc tp}, tc <= t -> tp <= t -> 
-      forall {r m}, marksend rch c p a tc r ->
-        marksend mch p c a tp m -> (forall tc', tc' < tc -> ~ recv mch p c a tc' m) ->
-        (forall tp', tp' <= tp -> ~ recv rch c p a tp' r) -> False.
-    Proof.
-      intros a t.
-      induction t.
-      intros tc tp tcLeT tpLeT r m rsendr msendm mrecvNo rrecvNo.
-      assert (tc0: tc = 0) by omega; clear tcLeT.
-      assert (tp0: tp = 0) by omega; clear tpLeT.
-      rewrite tc0 in *; rewrite tp0 in *; clear tc0 tp0.
-      pose proof (dirSendmImpRecvr msendm) as [r' rrecvr'].
-      pose proof (recvImpMarkSend rrecvr') as [t' [t'Le0 rsendr']].
-      assert (t'0: t' = 0) by omega; clear t'Le0.
-      rewrite t'0 in rsendr'; clear t'0.
-      pose proof (uniqMarksend1 rsendr rsendr') as rEqr'.
-      rewrite <- rEqr' in *; clear rEqr'.
-      assert (zero: 0 <= 0) by omega.
-      firstorder.
-      intros tc tp tcLeST tpLeST r m rsendr msendm mrecvNo rrecvNo.
+Module Type DirBase (dt: DataTypes) (p: Pair dt) (ch: ChannelPerAddr dt) (st: DirSemi dt p ch).
+  Module ll := LocalLemmas dt ch st.
+  Include ll.
+  Include st.
+  Import dt ch st p.
 
-      pose proof (dirSendmImpRecvr msendm) as [r' rrecvr'].
-      pose proof (recvImpMarkSend rrecvr') as [t' [t'LeSt rsendr']].
+  Section ForT.
+    Context {a: Addr} {t: Time}.
 
-      assert (diff: t' = tc \/ t' > tc \/ t' < tc) by omega.
-      destruct diff as [eq | [t'GtTc | tcGtT']].
-      rewrite eq in rsendr'.
-      pose proof (uniqMarksend1 rsendr rsendr') as rEqr'.
-      rewrite <- rEqr' in *.
-      assert (tpEq: tp <= tp) by omega.
-      firstorder.
+    Axiom sendmImpRecvr: forall {m}, marksend mch p c a t m -> exists r, recv rch c p a t r.
 
-      pose proof (sb.sendrImpNoSendr t'GtTc rsendr rsendr') as [t'' [cond neg]].
-      unfold St.toRSComp in *; unfold St.st in *; unfold St.rmarksend in *.
-      assert (toRLes: to r <= state c a t'') by firstorder.
-      pose proof (sb.sendrImpSt rsendr) as toGtt.
-      unfold St.toRSComp in *; unfold St.st in *.
-      assert (tcLtT'': state c a tc < state c a t'') by omega.
-      assert (t''GtTc: t'' > tc) by omega.
-      pose proof (whenChildHigh t''GtTc tcLtT'') as [t''' [[tcLeT''' t'''LtT''] [m' [mrecvm' _]]]].
-      pose proof (recvImpMarkSend mrecvm') as [td [tdLeT''' msendm']].
-      assert (tdLet: td <= t) by omega.
-      assert (noRecv: forall tc', tc' < tc -> ~ recv mch p c a tc' m') by (
-        unfold not; intros tc' tc'LtTc mrecvm'Tc';
-          pose proof (uniqRecv2 mrecvm' mrecvm'Tc') as tc'EqT''; omega).
-      assert (noRecv': forall tp', tp' <= td -> ~ recv rch c p a tp' r) by (
-        unfold not; intros tp' tp'LeTd;
-          assert (tp'LeTp: tp' <= tp) by omega;
-            firstorder).
-      assert (tcLeT: tc <= t) by omega.
-      apply (IHt tc td tcLeT tdLet r m' rsendr msendm' noRecv noRecv').
+    Axiom sendmImpRecvrGe: forall {m}, marksend mch p c a t m ->
+      forall {r}, recv rch c p a t r -> to m >= to r.
 
-      pose proof (sb.sendrImpNoSendr tcGtT' rsendr' rsendr) as [tmur [cond neg]].
-      (* unfold sb.isRMarksend in *. *)
-      unfold St.toRSComp in *; unfold St.st in *; unfold St.rmarksend in *.
-      assert (toRLeS: to r' <= state c a tmur) by omega.
-      pose proof (sb.sendrImpSt rsendr') as toGtt.
-      unfold St.toRSComp in *; unfold St.st in *.
-      assert (stt'LtstTc: state c a t' < state c a tmur) by omega.
-      assert (tmurGtT': tmur > t') by omega.
-      pose proof (whenChildHigh tmurGtT' stt'LtstTc) as [t'' [[tcLeT'' t''LtT'] [m' [mrecvm' _]]]].
-      pose proof (recvImpMarkSend mrecvm') as [td [tdLeT'' msendm']].
-      assert (tdLet: td <= t) by omega.
-      assert (noRecv: forall tc', tc' < t' -> ~ recv mch p c a tc' m') by (
-        unfold not; intros tc' tc'LtTc mrecvm'Tc';
-          pose proof (uniqRecv2 mrecvm' mrecvm'Tc') as tc'EqT''; omega).
-      assert (opts: td = tp \/ td < tp \/ td > tp) by omega.
-      destruct opts as [tdEqTp | [tdLTp | tdGtTp]].
-      rewrite tdEqTp in *.
-      pose proof (uniqMarksend1 msendm msendm') as mEqm'.
-      rewrite <- mEqm' in *.
-      assert (t''LtTc: t'' < tc) by omega.
-      firstorder.
-      assert (noRecv': forall tp', tp' <= td -> ~ recv rch c p a tp' r') by (
-        unfold not; intros tp' tp'LeTd rrecvr'Tp';
-          pose proof (uniqRecv2 rrecvr' rrecvr'Tp') as tp'EqTp;
-            omega).
-      assert (t'LeT: t' <= t) by omega.
-      apply (IHt t' td t'LeT tdLet r' m' rsendr' msendm' noRecv noRecv').
-      pose proof (dirSendmImpRecvr msendm') as [r'' rrecvr''].
-      pose proof (recvImpMarkSend rrecvr'') as [ts [tsLeTd rsendr'']].
-      assert (tpLeT: tp <= t) by omega.
-      assert (tsLeT: ts <= t) by omega.
-      assert (hyp1: forall tc', tc' < ts -> ~ recv mch p c a tc' m) by (
-        intros tc' tc'LtTs;
-          assert (tc'LtTc: tc' < tc) by omega;
-            firstorder).
-      assert (hyp2: forall tp', tp' <= tp -> ~ recv rch c p a tp' r'') by (
-        unfold not; intros tp' tpLeTp rrecvr''Tp';
-          pose proof (uniqRecv2 rrecvr'' rrecvr''Tp') as tdEqTp';
-            rewrite <- tdEqTp' in *;
-              firstorder).
-      apply (IHt ts tp tsLeT tpLeT r'' m rsendr'' msendm hyp1 hyp2).
-    Qed.
+    Axiom recvrCond: forall {r}, recv rch c p a t r -> from r >= dir p c a t.
 
-    Lemma cReqPRespCross: forall {a tc tp r m}, marksend rch c p a tc r ->
+    Axiom recvmCond: forall {m}, recv mch c p a t m -> from m = dir p c a t.
+
+    Axiom sendrImpNoSendm: forall {t1 t2 r1 m2}, t1 < t2 -> marksend rch p c a t1 r1 ->
+      marksend mch p c a t2 m2 ->
+      exists t', t1 < t' < t2 /\ exists m, recv mch c p a t' m /\ to m <= to r1.
+  End ForT.
+End DirBase.
+
+Module Dir (dt: DataTypes) (p: Pair dt) (ch: ChannelPerAddr dt) (d: DirSemi dt p ch) (db: DirBase dt p ch d)
+  (s: StSemi dt p ch) (sb: StBase dt p ch s).
+  Include db.
+  Import dt ch p.
+  
+  Lemma dirRecvImpLow: forall {a t m}, recv mch c p a t m -> dir p c a t > dir p c a (S t).
+  Proof.
+    intros a t m recvm.
+    pose proof (recvImpMarkSend recvm) as [t' [t'LeT sendm]].
+    pose proof (db.recvmChange recvm) as sth.
+    pose proof (sb.sendmImpSt sendm) as sth2.
+    pose proof (db.recvmCond recvm) as sth3.
+    pose proof (sb.sendmFrom sendm) as sth4.
+    unfold d.st, sb.st in *.
+    omega.
+  Qed.
+
+  Lemma whenDirLow': forall {a t t'}, dir p c a (t' + t) > dir p c a t ->
+    exists t'', t'' < t' /\ exists m, marksend mch p c a (t'' + t) m.
+  Proof.
+    intros a t t'.
+    induction t'.
+    intros dirGt.
+    unfold plus in *; simpl. omega.
+    intros dirGt.
+    assert (opts: dir p c a (t' + t) > dir p c a t \/ dir p c a (t' + t) <= dir p c a t) by omega.
+    destruct opts as [gt | le].
+    firstorder.
+    assert (gt: dir p c a (S (t' + t)) > dir p c a (t' + t)) by (assert (eq: S t' + t = S (t' + t)) by omega;
+      rewrite eq in *; omega).
+    assert (nestuff: dir p c a (S (t' + t)) <> dir p c a (t' + t)) by omega.
+    pose proof (db.change nestuff) as [sendm | recvm].
+    firstorder.
+    destruct recvm as [x recvstuff].
+    pose proof (dirRecvImpLow recvstuff) as contra.
+    omega.
+  Qed.
+
+  Lemma whenDirLow: forall {a t t1}, t <= t1 -> dir p c a t1 > dir p c a t ->
+    exists t'', t <= t'' < t1 /\ exists m, marksend mch p c a t'' m.
+  Proof.
+    intros a t t1 t1LeT1 dirGt.
+    assert (opt: t = t1 \/ t < t1) by omega.
+    destruct opt as [tEqT1 | tLeT1].
+    rewrite tEqT1 in *; omega.
+    remember (t1 - t - 1) as t'.
+    assert (eq: t1 = (t' + 1) + t) by omega.
+    rewrite eq in *.
+    pose proof (whenDirLow' dirGt) as [t'' [t''Cond ext]]. 
+    exists (t'' + t).
+    firstorder.
+  Qed.
+End Dir.
+
+Module Type PairProperties (dt: DataTypes) (ch: ChannelPerAddr dt) (p: Pair dt).
+  Import dt ch p.
+
+  Axiom init: forall {a}, dir p c a 0 = state c a 0.
+
+  Definition twoEqPRespFalse := forall a t t1 m1, t1 <= t -> marksend mch p c a t1 m1 ->
+    forall t2 m2, t2 <= t -> marksend mch p c a t2 m2 ->
+      (forall t3, t3 <= t -> ~ recv mch p c a t3 m1) -> (forall {t4}, t4 <= t -> ~ recv mch p c a t4 m2) ->
+      t1 = t2.
+
+  Definition twoPReqNeedsResp := forall a t t1 r1, t1 <= t -> marksend rch p c a t1 r1 -> forall t2 r2,
+    t2 <= t -> marksend rch p c a t2 r2 -> (forall t3, t3 <= t -> ~ recv rch p c a t3 r1) ->
+    (forall t4, t4 <= t -> ~ recv rch p c a t4 r2) -> to r1 = to r2 -> t1 < t2 ->
+    exists tm m, t1 < tm < t2 /\ marksend mch p c a tm m.
+
+  Section ForA.
+    Context {a: Addr}.
+    Axiom pRespReq: twoEqPRespFalse -> twoPReqNeedsResp -> forall {t1 t2 t3},
+      forall {m}, marksend mch p c a t1 m ->
+        forall {r}, marksend rch p c a t2 r -> recv rch p c a t3 r -> t1 <= t2 ->
+          exists t4, t4 < t3 /\ recv mch p c a t4 m.
+
+    Axiom pReqResp: twoEqPRespFalse -> twoPReqNeedsResp -> forall {t1 t2 t3},
+      forall {r}, marksend rch p c a t1 r ->
+        forall {m}, marksend mch p c a t2 m -> recv mch p c a t3 m -> t1 <= t2 ->
+          exists t4, t4 < t3 /\ recv rch p c a t4 r.
+  End ForA.
+End PairProperties.
+
+Module Type PairTheoremsType (dt: DataTypes) (ch: ChannelPerAddr dt) (p: Pair dt)
+  (pp: PairProperties dt ch p).
+  Import dt ch p pp.
+
+  Axiom noTwoPResp: twoEqPRespFalse.
+  Axiom noTwoPReqNon: twoPReqNeedsResp.
+
+  Axiom conservative: forall {a t}, dir p c a t >= state c a t.
+  Axiom cReqRespSent: forall {a t1 t2 r}, marksend rch p c a t1 r -> recv rch p c a t2 r ->
+    to r >= state c a t2 -> exists t3, t3 < t2 /\ exists m, marksend mch c p a t3 m /\ to m <= to r /\
+      (forall t4, t4 < t1 -> ~ recv mch c p a t4 m).
+End PairTheoremsType.
+
+Module Type Classical.
+  Axiom classical: forall P, P \/ ~ P.
+End Classical.
+
+Module PairTheorems (classical: Classical) (dt: DataTypes) (ch: ChannelPerAddr dt)
+  (p: Pair dt) (pp: PairProperties dt ch p)
+  (stSemi: StSemi dt p ch) (dirSemi: DirSemi dt p ch) (stBase: StBase dt p ch stSemi)
+  (dirBase: DirBase dt p ch dirSemi): PairTheoremsType dt ch p pp.
+  Module st := St dt p ch stSemi stBase.
+  Module dir := Dir dt p ch dirSemi dirBase stSemi stBase.
+  Import dt ch p pp.
+
+  Lemma cReqPRespCrossInd: forall {a t tc tp}, tc <= t -> tp <= t -> 
+    forall {r m}, marksend rch c p a tc r ->
       marksend mch p c a tp m -> (forall tc', tc' < tc -> ~ recv mch p c a tc' m) ->
       (forall tp', tp' <= tp -> ~ recv rch c p a tp' r) -> False.
-    Proof.
-      intros a tc tp.
-      assert (tcLeT: tc <= tc + tp) by omega.
-      assert (tpLeT: tp <= tc + tp) by omega.
-      apply (@cReqPRespCrossInd a (tc + tp) tc tp tcLeT tpLeT).
-    Qed.
+  Proof.
+    intros a t.
+    induction t.
+    intros tc tp tcLeT tpLeT r m rsendr msendm mrecvNo rrecvNo.
+    assert (tc0: tc = 0) by omega; clear tcLeT.
+    assert (tp0: tp = 0) by omega; clear tpLeT.
+    rewrite tc0 in *; rewrite tp0 in *; clear tc0 tp0.
+    pose proof (dir.sendmImpRecvr msendm) as [r' rrecvr'].
+    pose proof (recvImpMarkSend rrecvr') as [t' [t'Le0 rsendr']].
+    assert (t'0: t' = 0) by omega; clear t'Le0.
+    rewrite t'0 in rsendr'; clear t'0.
+    pose proof (uniqMarksend1 rsendr rsendr') as rEqr'.
+    rewrite <- rEqr' in *; clear rEqr'.
+    assert (zero: 0 <= 0) by omega.
+    firstorder.
+    intros tc tp tcLeST tpLeST r m rsendr msendm mrecvNo rrecvNo.
 
-    Lemma noTwoPResp: twoEqPRespFalse.
-    Proof.
-      intros a tx t1 m1 t1LeTx sendm1 t2 m2 t2LeTx sendm2 norecvm1 norecvm2.
-      pose proof (dirSendmImpRecvr sendm1) as [r1 recvr1].
-      pose proof (dirSendmImpRecvr sendm2) as [r2 recvr2].
-      pose proof (recvImpMarkSend recvr1) as [t3 [t3LeT1 sendr1]].
-      pose proof (recvImpMarkSend recvr2) as [t4 [t4LeT2 sendr2]].
-      assert (opts: t3 = t4 \/ t3 < t4 \/ t4 < t3) by omega.
-      destruct opts as [t3EqT4|[t3LtT4|t4LtT3]].
-      rewrite t3EqT4 in *; pose proof (uniqMarksend1 sendr1 sendr2) as r1EqR2.
-      rewrite r1EqR2 in *; apply (uniqRecv2 recvr1 recvr2).
+    pose proof (dir.sendmImpRecvr msendm) as [r' rrecvr'].
+    pose proof (recvImpMarkSend rrecvr') as [t' [t'LeSt rsendr']].
 
-      assert (noRecv: ~ exists t, t3 <= t < t4 /\ exists m, recv mch p c a t m) by (
-        unfold not; intros [t [cond [m recvm]]];
-          pose proof (recvImpMarkSend recvm) as [t5 [t5LeT sendm]];
-            assert (opts: t5 = t1 \/ t5 < t1 \/ t5 > t1) by omega;
-              destruct opts as [t5EqT1 | [t5LtT1 | t5GtT1]]; [
-                rewrite t5EqT1 in *; pose proof (uniqMarksend1 sendm1 sendm) as m1EqM;
-                  rewrite m1EqM in *; assert (tLeTx: t <= tx) by omega;
-                    generalize tLeTx norecvm1 recvm; clear; firstorder |
-                assert (one: forall tc', tc' < t3 -> ~ recv mch p c a tc' m) by (
-                  unfold not; intros tc' tc'LtT3 recv'm; pose proof (uniqRecv2 recvm recv'm) as tEqTc';
-                    rewrite tEqTc' in *; firstorder);
-                assert (two: forall tp', tp' <= t5 -> ~ recv rch c p a tp' r1) by (
-                  unfold not; intros tp' tp'LeT1 recv'r1; pose proof (uniqRecv2 recvr1 recv'r1) as t5EqTp';
-                    rewrite <- t5EqTp' in *; firstorder);
-                apply (cReqPRespCross sendr1 sendm one two) |
-                  pose proof (dirSendmImpRecvr sendm) as [r recvr];
-                    pose proof (recvImpMarkSend recvr) as [t6 [t6LeT5 sendr]];
-                      assert (one: forall tc', tc' < t6 -> ~ recv mch p c a tc' m1) by (
-                        unfold not; intros tc' tc'LtT6 recv'm1; assert (tc'LeT6: tc' <= tx) by omega;
-                          generalize norecvm1 recv'm1 tc'LeT6; clear; firstorder);
-                      assert (two: forall tp', tp' <= t1 -> ~ recv rch c p a tp' r) by (
-                        unfold not; intros tp' tp'LeT1 recv'r; pose proof (uniqRecv2 recvr recv'r) as t1EqTp';
-                          rewrite <- t1EqTp' in *; firstorder);
-                      apply (cReqPRespCross sendr sendm1 one two)]).
-      assert (t3LeT4: t3 <= t4) by omega.
-      pose proof (sb.sendrImpSt sendr1) as stG. unfold St.st, St.toRSComp in *.
-      pose proof (sb.sendrImpNoSendr t3LtT4 sendr1 sendr2) as [t5 [t3LtT5LeT4 neg]].
-      unfold St.toRSComp, St.st in *.
-      assert (pos: state c a t5 > state c a t3) by omega.
-      assert (noRecv': ~ exists t, t3 <= t < t5 /\ exists m, recv mch p c a t m /\ to m >= state c a t5) by (
-        unfold not; intros [t [cond1 [mg [recvmg _]]]];
-          assert (cond: t3 <= t < t4) by omega;
-            generalize recvmg cond noRecv; clear; firstorder).
-      assert (t3LeT5: t3 <= t5) by omega.
-      pose proof (whenChildHighConv t3LeT5 noRecv') as stContra.
-      omega.
+    assert (diff: t' = tc \/ t' > tc \/ t' < tc) by omega.
+    destruct diff as [eq | [t'GtTc | tcGtT']].
+    rewrite eq in rsendr'.
+    pose proof (uniqMarksend1 rsendr rsendr') as rEqr'.
+    rewrite <- rEqr' in *.
+    assert (tpEq: tp <= tp) by omega.
+    firstorder.
 
-      assert (noRecv: ~ exists t, t4 <= t < t3 /\ exists m, recv mch p c a t m) by (
-        unfold not; intros [t [cond [m recvm]]];
-          pose proof (recvImpMarkSend recvm) as [t5 [t5LeT sendm]];
-            assert (opts: t5 = t2 \/ t5 < t2 \/ t5 > t2) by omega;
-              destruct opts as [t5EqT1 | [t5LtT1 | t5GtT1]]; [
-                rewrite t5EqT1 in *; pose proof (uniqMarksend1 sendm2 sendm) as m1EqM;
-                  rewrite m1EqM in *; assert (tLeTx: t <= tx) by omega;
-                    generalize tLeTx norecvm2 recvm; clear; firstorder |
-                assert (one: forall tc', tc' < t4 -> ~ recv mch p c a tc' m) by (
-                  unfold not; intros tc' tc'LtT3 recv'm; pose proof (uniqRecv2 recvm recv'm) as tEqTc';
-                    rewrite tEqTc' in *; firstorder);
-                assert (two: forall tp', tp' <= t5 -> ~ recv rch c p a tp' r2) by (
-                  unfold not; intros tp' tp'LeT1 recv'r1; pose proof (uniqRecv2 recvr2 recv'r1) as t5EqTp';
-                    rewrite <- t5EqTp' in *; firstorder);
-                apply (cReqPRespCross sendr2 sendm one two)|
-                  pose proof (dirSendmImpRecvr sendm) as [r recvr];
-                    pose proof (recvImpMarkSend recvr) as [t6 [t6LeT5 sendr]];
-                      assert (one: forall tc', tc' < t6 -> ~ recv mch p c a tc' m2) by (
-                        unfold not; intros tc' tc'LtT6 recv'm1; assert (tc'LeT6: tc' <= tx) by omega;
-                          generalize norecvm2 recv'm1 tc'LeT6; clear; firstorder);
-                      assert (two: forall tp', tp' <= t2 -> ~ recv rch c p a tp' r) by (
-                        unfold not; intros tp' tp'LeT1 recv'r; pose proof (uniqRecv2 recvr recv'r) as t1EqTp';
-                          rewrite <- t1EqTp' in *; firstorder);
-                      apply (cReqPRespCross sendr sendm2 one two)]).
-      assert (t3LeT4: t4 <= t3) by omega.
-      pose proof (sb.sendrImpSt sendr2) as stG. unfold St.st, St.toRSComp in *.
-      pose proof (sb.sendrImpNoSendr t4LtT3 sendr2 sendr1) as [t5 [t3LtT5LeT4 neg]].
-      unfold St.toRSComp, St.st in *.
-      assert (pos: state c a t5 > state c a t4) by omega.
-      assert (noRecv': ~ exists t, t4 <= t < t5 /\ exists m, recv mch p c a t m /\ to m >= state c a t5) by (
-        unfold not; intros [t [cond1 [mg [recvmg _]]]];
-          assert (cond: t4 <= t < t3) by omega;
-            generalize recvmg cond noRecv; clear; firstorder).
-      assert (t3LeT5: t4 <= t5) by omega.
-      pose proof (whenChildHighConv t3LeT5 noRecv') as stContra.
-      omega.
-    Qed.
+    pose proof (st.sendrImpNoSendr t'GtTc rsendr rsendr') as [t'' [cond neg]].
+    unfold st.toRSComp in *; unfold st.st in *.
+    assert (toRLes: to r <= state c a t'') by firstorder.
+    pose proof (st.sendrImpSt rsendr) as toGtt.
+    unfold st.toRSComp in *; unfold st.st in *.
+    assert (tcLtT'': state c a tc < state c a t'') by omega.
+    assert (t''GtTc: t'' > tc) by omega.
+    pose proof (st.whenChildHigh t''GtTc tcLtT'') as [t''' [[tcLeT''' t'''LtT''] [m' [mrecvm' _]]]].
+    pose proof (recvImpMarkSend mrecvm') as [td [tdLeT''' msendm']].
+    assert (tdLet: td <= t) by omega.
+    assert (noRecv: forall tc', tc' < tc -> ~ recv mch p c a tc' m') by (
+      unfold not; intros tc' tc'LtTc mrecvm'Tc';
+        pose proof (uniqRecv2 mrecvm' mrecvm'Tc') as tc'EqT''; omega).
+    assert (noRecv': forall tp', tp' <= td -> ~ recv rch c p a tp' r) by (
+      unfold not; intros tp' tp'LeTd;
+        assert (tp'LeTp: tp' <= tp) by omega;
+          firstorder).
+    assert (tcLeT: tc <= t) by omega.
+    apply (IHt tc td tcLeT tdLet r m' rsendr msendm' noRecv noRecv').
 
-    Lemma noTwoPReqNon: twoPReqNeedsResp.
-    Proof.
-      intros a t t1 r1 t1LeT sendr1 t2 r2 t2LeT sendr2 norecvr1 norecvr2 toR1EqToR2 t1LtT2.
-      pose proof (db.sendrImpSt sendr1) as gt1.
-      pose proof (db.sendrImpSt sendr2) as gt2.
-      unfold Dir.toRSComp, Dir.st, Dir.rmarksend in *.
-      pose proof (db.sendrImpNoSendr t1LtT2 sendr1 sendr2) as [t5 [cond dr]].
-      unfold Dir.st, Dir.toRSComp in *.
-      assert (toR1GeDirT5: to r1 >= dir p c a t5) by omega; clear dr.
-      assert (dT5LtDt2: dir p c a t5 < dir p c a t2) by omega.
-      assert (t5LeT2: t5 <= t2) by omega.
-      pose proof (whenDirLow t5LeT2 dT5LtDt2) as [tm [m [cond2 sendm]]].
-      assert (cond3: t1 < tm < t2) by omega.
-      firstorder.
-    Qed.
+    pose proof (st.sendrImpNoSendr tcGtT' rsendr' rsendr) as [tmur [cond neg]].
+    unfold st.toRSComp in *; unfold st.st in *.
+    assert (toRLeS: to r' <= state c a tmur) by omega.
+    pose proof (st.sendrImpSt rsendr') as toGtt.
+    unfold st.toRSComp in *; unfold st.st in *.
+    assert (stt'LtstTc: state c a t' < state c a tmur) by omega.
+    assert (tmurGtT': tmur > t') by omega.
+    pose proof (st.whenChildHigh tmurGtT' stt'LtstTc) as [t'' [[tcLeT'' t''LtT'] [m' [mrecvm' _]]]].
+    pose proof (recvImpMarkSend mrecvm') as [td [tdLeT'' msendm']].
+    assert (tdLet: td <= t) by omega.
+    assert (noRecv: forall tc', tc' < t' -> ~ recv mch p c a tc' m') by (
+      unfold not; intros tc' tc'LtTc mrecvm'Tc';
+        pose proof (uniqRecv2 mrecvm' mrecvm'Tc') as tc'EqT''; omega).
+    assert (opts: td = tp \/ td < tp \/ td > tp) by omega.
+    destruct opts as [tdEqTp | [tdLTp | tdGtTp]].
+    rewrite tdEqTp in *.
+    pose proof (uniqMarksend1 msendm msendm') as mEqm'.
+    rewrite <- mEqm' in *.
+    assert (t''LtTc: t'' < tc) by omega.
+    firstorder.
+    assert (noRecv': forall tp', tp' <= td -> ~ recv rch c p a tp' r') by (
+      unfold not; intros tp' tp'LeTd rrecvr'Tp';
+        pose proof (uniqRecv2 rrecvr' rrecvr'Tp') as tp'EqTp;
+          omega).
+    assert (t'LeT: t' <= t) by omega.
+    apply (IHt t' td t'LeT tdLet r' m' rsendr' msendm' noRecv noRecv').
+    pose proof (dir.sendmImpRecvr msendm') as [r'' rrecvr''].
+    pose proof (recvImpMarkSend rrecvr'') as [ts [tsLeTd rsendr'']].
+    assert (tpLeT: tp <= t) by omega.
+    assert (tsLeT: ts <= t) by omega.
+    assert (hyp1: forall tc', tc' < ts -> ~ recv mch p c a tc' m) by (
+      intros tc' tc'LtTs;
+        assert (tc'LtTc: tc' < tc) by omega;
+          firstorder).
+    assert (hyp2: forall tp', tp' <= tp -> ~ recv rch c p a tp' r'') by (
+      unfold not; intros tp' tpLeTp rrecvr''Tp';
+        pose proof (uniqRecv2 rrecvr'' rrecvr''Tp') as tdEqTp';
+          rewrite <- tdEqTp' in *;
+            firstorder).
+    apply (IHt ts tp tsLeT tpLeT r'' m rsendr'' msendm hyp1 hyp2).
+  Qed.
 
-    Lemma mainInd: forall {a t},
-      (forall {to}, to <= t -> state c a to <= dir p c a to) /\
-      (forall {tc tp}, tc <= t -> tp <= t -> forall {mc}, marksend mch c p a tc mc ->
-        forall {mp}, marksend mch p c a tp mp -> (forall tc', tc' < tc -> ~ recv mch p c a tc' mp) ->
-          (forall tp', tp' < tp -> ~ recv mch c p a tp' mc) -> False) /\
-       (forall {t1 t2 t3}, t3 <= t -> forall {m}, marksend mch c p a t1 m ->
-         forall {r}, marksend rch c p a t2 r -> recv rch c p a t3 r -> t1 <= t2 ->
-          (forall t4, t4 < t3 -> ~ recv mch c p a t4 m) -> False) /\
-       (forall {t1 t2 t3}, t3 <= t -> forall {m}, marksend mch c p a t1 m ->
-         forall {m'}, marksend mch c p a t2 m' -> recv mch c p a t3 m' -> t1 < t2 ->
-          (forall t4, t4 < t3 -> ~ recv mch c p a t4 m) -> False).
-    Proof.
-      intros a t.
-      induction t.
-      constructor.
-      intros to0 to0Le0.
-      assert (to0Eq0: to0 = 0) by omega.
-      pose proof (init a) as start.
-      rewrite to0Eq0.
-      omega.
-      constructor.
-      intros tc tp tcLe0 tpLe0 mc msendmc mp msendmp _ _.
-      assert (tcEq0: tc = 0) by omega; assert (tpEq0: tp = 0) by omega.
-      rewrite tcEq0 in *; rewrite tpEq0 in *.
-      pose proof (dirSendmImpRecvr msendmp) as [r rrecvr].
-      pose proof (recvImpMarkSend rrecvr) as [t' [t'Le0 rsendr]].
-      assert (t'Eq0: t' = 0) by omega.
-      rewrite t'Eq0 in *.
-      apply (sb.noSendmSendr msendmc rsendr).
-      constructor.
-      intros t1 t2 t3 t3Le0 m msendm r rsendr rrecvr t1LeT2 neg.
-      pose proof (recvImpMarkSend rrecvr) as [t5 [t5LeT3 rsendrT5]].
-      pose proof (uniqMarksend2 rsendr rsendrT5) as t2EqT5.
-      assert (t30: t3 = 0) by omega.
-      rewrite t2EqT5, t30 in *.
-      assert (t1Le0: t1 <= 0) by omega.
-      assert (t10: t1 = 0) by intuition.
-      assert (t50: t5 = 0) by omega.
-      rewrite t10, t50 in *.
-      apply (sb.noSendmSendr msendm rsendr).
-      intros t1 t2 t3 t3Le0 m msendm m' msendm' mrecvm' t1LeT2 neg.
-      pose proof (recvImpMarkSend mrecvm') as [t5 [t5LeT3 msendm'T5]].
-      pose proof (uniqMarksend2 msendm' msendm'T5) as t2EqT5.
-      assert (t30: t3 = 0) by omega.
-      rewrite t2EqT5, t30 in *.
-      assert (t1Le0: t1 <= 0) by omega.
-      assert (t10: t1 = 0) by intuition.
-      assert (t50: t5 = 0) by omega.
-      rewrite t10, t50 in *.
-      omega.
-      
-      destruct IHt as [cons [cross [cReqResp cRespResp]]].
+  Lemma cReqPRespCross: forall {a tc tp r m}, marksend rch c p a tc r ->
+    marksend mch p c a tp m -> (forall tc', tc' < tc -> ~ recv mch p c a tc' m) ->
+    (forall tp', tp' <= tp -> ~ recv rch c p a tp' r) -> False.
+  Proof.
+    intros a tc tp.
+    assert (tcLeT: tc <= tc + tp) by omega.
+    assert (tpLeT: tp <= tc + tp) by omega.
+    apply (@cReqPRespCrossInd a (tc + tp) tc tp tcLeT tpLeT).
+  Qed.
 
-      assert (cross': forall to0, to0 <= S t -> state c a to0 <= dir p c a to0).
-      intros tm toLtT.
-      destruct (classical (exists ts, ts < tm /\ ((exists m, recv mch c p a ts m) \/
-        (exists m, marksend mch p c a ts m)))) as [chnge|noChnge].
-      pose proof (maxExists' classical chnge) as lastChnge; clear chnge.
-      destruct lastChnge as [ts [tsLtTo [recvOrSend noPrevChnge]]].
-      assert (eq: dir p c a (S ts) = dir p c a tm) by (
-        assert (two: S ts = tm \/ S ts < tm) by omega;
-          destruct two as [eq|less]; [
-            intuition|
-              apply db.noChange; [ intuition | generalize noPrevChnge; clear; firstorder]]).
-      destruct recvOrSend as [[m mrecvm] | [m msendm]].
-      pose proof (recvImpMarkSend mrecvm) as [t' [t'LeTs msendm]].
-      destruct (classical (exists tc, t' < tc < tm /\ exists m, recv mch p c a tc m)) as [recv|noRecv].
-      destruct recv as [tc [comp [m' mrecvm']]].
-      pose proof (recvImpMarkSend mrecvm') as [t'' [t''LeTc msendm']].
-      assert (gOrl: t'' > ts \/ t'' <= ts) by omega.
-      destruct gOrl as [t''GtTs | t''LeTs].
-      assert (t''LtTc: t'' < tm) by omega.
-      generalize noPrevChnge msendm' t''LtTc t''GtTs; clear; firstorder.
-      assert (t'LeT: t' <= t) by omega.
-      assert (t''LeT: t'' <= t) by omega.
-      assert (hyp1: forall tc', tc' < t' -> ~ recv mch p c a tc' m') by (
-        unfold not; intros tc' tc'LtT' mrecvm'Tc';
-          pose proof (uniqRecv2 mrecvm' mrecvm'Tc'); intuition).
-      assert (hyp2: forall tp', tp' < t'' -> ~ recv mch c p a tp' m) by (
-        unfold not; intros tp' tp'LtT'' mrecvmTp';
-          pose proof (uniqRecv2 mrecvm mrecvmTp'); intuition).
-      pose proof (cross t' t'' t'LeT t''LeT m msendm m' msendm' hyp1 hyp2).
-      firstorder.
-      assert (noRecv': ~ (exists tc, S t' <= tc < tm /\ exists m, recv mch p c a tc m /\ to m >= state c a tm)) by
-        (
+  Lemma noTwoPResp: twoEqPRespFalse.
+  Proof.
+    intros a tx t1 m1 t1LeTx sendm1 t2 m2 t2LeTx sendm2 norecvm1 norecvm2.
+    pose proof (dir.sendmImpRecvr sendm1) as [r1 recvr1].
+    pose proof (dir.sendmImpRecvr sendm2) as [r2 recvr2].
+    pose proof (recvImpMarkSend recvr1) as [t3 [t3LeT1 sendr1]].
+    pose proof (recvImpMarkSend recvr2) as [t4 [t4LeT2 sendr2]].
+    assert (opts: t3 = t4 \/ t3 < t4 \/ t4 < t3) by omega.
+    destruct opts as [t3EqT4|[t3LtT4|t4LtT3]].
+    rewrite t3EqT4 in *; pose proof (uniqMarksend1 sendr1 sendr2) as r1EqR2.
+    rewrite r1EqR2 in *; apply (uniqRecv2 recvr1 recvr2).
+
+    assert (noRecv: ~ exists t, t3 <= t < t4 /\ exists m, recv mch p c a t m) by (
+      unfold not; intros [t [cond [m recvm]]];
+        pose proof (recvImpMarkSend recvm) as [t5 [t5LeT sendm]];
+          assert (opts: t5 = t1 \/ t5 < t1 \/ t5 > t1) by omega;
+            destruct opts as [t5EqT1 | [t5LtT1 | t5GtT1]]; [
+              rewrite t5EqT1 in *; pose proof (uniqMarksend1 sendm1 sendm) as m1EqM;
+                rewrite m1EqM in *; assert (tLeTx: t <= tx) by omega;
+                  generalize tLeTx norecvm1 recvm; clear; firstorder |
+                    assert (one: forall tc', tc' < t3 -> ~ recv mch p c a tc' m) by (
+                      unfold not; intros tc' tc'LtT3 recv'm; pose proof (uniqRecv2 recvm recv'm) as tEqTc';
+                        rewrite tEqTc' in *; firstorder);
+                    assert (two: forall tp', tp' <= t5 -> ~ recv rch c p a tp' r1) by (
+                      unfold not; intros tp' tp'LeT1 recv'r1; pose proof (uniqRecv2 recvr1 recv'r1) as t5EqTp';
+                        rewrite <- t5EqTp' in *; firstorder);
+                    apply (cReqPRespCross sendr1 sendm one two) |
+                      pose proof (dir.sendmImpRecvr sendm) as [r recvr];
+                        pose proof (recvImpMarkSend recvr) as [t6 [t6LeT5 sendr]];
+                          assert (one: forall tc', tc' < t6 -> ~ recv mch p c a tc' m1) by (
+                            unfold not; intros tc' tc'LtT6 recv'm1; assert (tc'LeT6: tc' <= tx) by omega;
+                              generalize norecvm1 recv'm1 tc'LeT6; clear; firstorder);
+                          assert (two: forall tp', tp' <= t1 -> ~ recv rch c p a tp' r) by (
+                            unfold not; intros tp' tp'LeT1 recv'r; pose proof (uniqRecv2 recvr recv'r) as t1EqTp';
+                              rewrite <- t1EqTp' in *; firstorder);
+                          apply (cReqPRespCross sendr sendm1 one two)]).
+    assert (t3LeT4: t3 <= t4) by omega.
+    pose proof (st.sendrImpSt sendr1) as stG. unfold st.st, st.toRSComp in *.
+    pose proof (st.sendrImpNoSendr t3LtT4 sendr1 sendr2) as [t5 [t3LtT5LeT4 neg]].
+    unfold st.toRSComp, st.st in *.
+    assert (pos: state c a t5 > state c a t3) by omega.
+    assert (noRecv': ~ exists t, t3 <= t < t5 /\ exists m, recv mch p c a t m /\ to m >= state c a t5) by (
+      unfold not; intros [t [cond1 [mg [recvmg _]]]];
+        assert (cond: t3 <= t < t4) by omega;
+          generalize recvmg cond noRecv; clear; firstorder).
+    assert (t3LeT5: t3 <= t5) by omega.
+    pose proof (st.whenChildHighConv t3LeT5 noRecv') as stContra.
+    omega.
+
+    assert (noRecv: ~ exists t, t4 <= t < t3 /\ exists m, recv mch p c a t m) by (
+      unfold not; intros [t [cond [m recvm]]];
+        pose proof (recvImpMarkSend recvm) as [t5 [t5LeT sendm]];
+          assert (opts: t5 = t2 \/ t5 < t2 \/ t5 > t2) by omega;
+            destruct opts as [t5EqT1 | [t5LtT1 | t5GtT1]]; [
+              rewrite t5EqT1 in *; pose proof (uniqMarksend1 sendm2 sendm) as m1EqM;
+                rewrite m1EqM in *; assert (tLeTx: t <= tx) by omega;
+                  generalize tLeTx norecvm2 recvm; clear; firstorder |
+                    assert (one: forall tc', tc' < t4 -> ~ recv mch p c a tc' m) by (
+                      unfold not; intros tc' tc'LtT3 recv'm; pose proof (uniqRecv2 recvm recv'm) as tEqTc';
+                        rewrite tEqTc' in *; firstorder);
+                    assert (two: forall tp', tp' <= t5 -> ~ recv rch c p a tp' r2) by (
+                      unfold not; intros tp' tp'LeT1 recv'r1; pose proof (uniqRecv2 recvr2 recv'r1) as t5EqTp';
+                        rewrite <- t5EqTp' in *; firstorder);
+                    apply (cReqPRespCross sendr2 sendm one two)|
+                      pose proof (dir.sendmImpRecvr sendm) as [r recvr];
+                        pose proof (recvImpMarkSend recvr) as [t6 [t6LeT5 sendr]];
+                          assert (one: forall tc', tc' < t6 -> ~ recv mch p c a tc' m2) by (
+                            unfold not; intros tc' tc'LtT6 recv'm1; assert (tc'LeT6: tc' <= tx) by omega;
+                              generalize norecvm2 recv'm1 tc'LeT6; clear; firstorder);
+                          assert (two: forall tp', tp' <= t2 -> ~ recv rch c p a tp' r) by (
+                            unfold not; intros tp' tp'LeT1 recv'r; pose proof (uniqRecv2 recvr recv'r) as t1EqTp';
+                              rewrite <- t1EqTp' in *; firstorder);
+                          apply (cReqPRespCross sendr sendm2 one two)]).
+    assert (t3LeT4: t4 <= t3) by omega.
+    pose proof (st.sendrImpSt sendr2) as stG. unfold st.st, st.toRSComp in *.
+    pose proof (st.sendrImpNoSendr t4LtT3 sendr2 sendr1) as [t5 [t3LtT5LeT4 neg]].
+    unfold st.toRSComp, st.st in *.
+    assert (pos: state c a t5 > state c a t4) by omega.
+    assert (noRecv': ~ exists t, t4 <= t < t5 /\ exists m, recv mch p c a t m /\ to m >= state c a t5) by (
+      unfold not; intros [t [cond1 [mg [recvmg _]]]];
+        assert (cond: t4 <= t < t3) by omega;
+          generalize recvmg cond noRecv; clear; firstorder).
+    assert (t3LeT5: t4 <= t5) by omega.
+    pose proof (st.whenChildHighConv t3LeT5 noRecv') as stContra.
+    omega.
+  Qed.
+
+  Lemma noTwoPReqNon: twoPReqNeedsResp.
+  Proof.
+    intros a t t1 r1 t1LeT sendr1 t2 r2 t2LeT sendr2 norecvr1 norecvr2 toR1EqToR2 t1LtT2.
+    pose proof (dir.sendrImpSt sendr1) as gt1.
+    pose proof (dir.sendrImpSt sendr2) as gt2.
+    unfold dir.toRSComp, dir.st.
+    pose proof (dir.sendrImpNoSendr t1LtT2 sendr1 sendr2) as [t5 [cond dr]].
+    unfold dir.st, dir.toRSComp in *.
+    assert (toR1GeDirT5: to r1 >= dir p c a t5) by omega; clear dr.
+    assert (dT5LtDt2: dir p c a t5 < dir p c a t2) by omega.
+    assert (t5LeT2: t5 <= t2) by omega.
+    pose proof (dir.whenDirLow t5LeT2 dT5LtDt2) as [tm [m [cond2 sendm]]].
+    assert (cond3: t1 < tm < t2) by omega.
+    firstorder.
+  Qed.
+
+  Import classical.
+  Lemma mainInd: forall {a t},
+    (forall {to}, to <= t -> state c a to <= dir p c a to) /\
+    (forall {tc tp}, tc <= t -> tp <= t -> forall {mc}, marksend mch c p a tc mc ->
+      forall {mp}, marksend mch p c a tp mp -> (forall tc', tc' < tc -> ~ recv mch p c a tc' mp) ->
+        (forall tp', tp' < tp -> ~ recv mch c p a tp' mc) -> False) /\
+    (forall {t1 t2 t3}, t3 <= t -> forall {m}, marksend mch c p a t1 m ->
+      forall {r}, marksend rch c p a t2 r -> recv rch c p a t3 r -> t1 <= t2 ->
+        (forall t4, t4 < t3 -> ~ recv mch c p a t4 m) -> False) /\
+    (forall {t1 t2 t3}, t3 <= t -> forall {m}, marksend mch c p a t1 m ->
+      forall {m'}, marksend mch c p a t2 m' -> recv mch c p a t3 m' -> t1 < t2 ->
+        (forall t4, t4 < t3 -> ~ recv mch c p a t4 m) -> False).
+  Proof.
+    intros a t.
+    induction t.
+    constructor.
+    intros to0 to0Le0.
+    assert (to0Eq0: to0 = 0) by omega.
+    pose proof (@init a) as start.
+    rewrite to0Eq0.
+    omega.
+    constructor.
+    intros tc tp tcLe0 tpLe0 mc msendmc mp msendmp _ _.
+    assert (tcEq0: tc = 0) by omega; assert (tpEq0: tp = 0) by omega.
+    rewrite tcEq0 in *; rewrite tpEq0 in *.
+    pose proof (dir.sendmImpRecvr msendmp) as [r rrecvr].
+    pose proof (recvImpMarkSend rrecvr) as [t' [t'Le0 rsendr]].
+    assert (t'Eq0: t' = 0) by omega.
+    rewrite t'Eq0 in *.
+    apply (st.noSendmSendr msendmc rsendr).
+    constructor.
+    intros t1 t2 t3 t3Le0 m msendm r rsendr rrecvr t1LeT2 neg.
+    pose proof (recvImpMarkSend rrecvr) as [t5 [t5LeT3 rsendrT5]].
+    pose proof (uniqMarksend2 rsendr rsendrT5) as t2EqT5.
+    assert (t30: t3 = 0) by omega.
+    rewrite t2EqT5, t30 in *.
+    assert (t1Le0: t1 <= 0) by omega.
+    assert (t10: t1 = 0) by intuition.
+    assert (t50: t5 = 0) by omega.
+    rewrite t10, t50 in *.
+    apply (st.noSendmSendr msendm rsendr).
+    intros t1 t2 t3 t3Le0 m msendm m' msendm' mrecvm' t1LeT2 neg.
+    pose proof (recvImpMarkSend mrecvm') as [t5 [t5LeT3 msendm'T5]].
+    pose proof (uniqMarksend2 msendm' msendm'T5) as t2EqT5.
+    assert (t30: t3 = 0) by omega.
+    rewrite t2EqT5, t30 in *.
+    assert (t1Le0: t1 <= 0) by omega.
+    assert (t10: t1 = 0) by intuition.
+    assert (t50: t5 = 0) by omega.
+    rewrite t10, t50 in *.
+    omega.
+    
+    destruct IHt as [cons [cross [cReqResp cRespResp]]].
+
+    assert (cross': forall to0, to0 <= S t -> state c a to0 <= dir p c a to0).
+    intros tm toLtT.
+    destruct (classical (exists ts, ts < tm /\ ((exists m, recv mch c p a ts m) \/
+      (exists m, marksend mch p c a ts m)))) as [chnge|noChnge].
+    pose proof (maxExists' classical chnge) as lastChnge; clear chnge.
+    destruct lastChnge as [ts [tsLtTo [recvOrSend noPrevChnge]]].
+    assert (eq: dir p c a (S ts) = dir p c a tm) by (
+      assert (two: S ts = tm \/ S ts < tm) by omega;
+        destruct two as [eq|less]; [
+          intuition|
+            apply dir.noChange; [ intuition | generalize noPrevChnge; clear; firstorder]]).
+    destruct recvOrSend as [[m mrecvm] | [m msendm]].
+    pose proof (recvImpMarkSend mrecvm) as [t' [t'LeTs msendm]].
+    destruct (classical (exists tc, t' < tc < tm /\ exists m, recv mch p c a tc m)) as [recv|noRecv].
+    destruct recv as [tc [comp [m' mrecvm']]].
+    pose proof (recvImpMarkSend mrecvm') as [t'' [t''LeTc msendm']].
+    assert (gOrl: t'' > ts \/ t'' <= ts) by omega.
+    destruct gOrl as [t''GtTs | t''LeTs].
+    assert (t''LtTc: t'' < tm) by omega.
+    generalize noPrevChnge msendm' t''LtTc t''GtTs; clear; firstorder.
+    assert (t'LeT: t' <= t) by omega.
+    assert (t''LeT: t'' <= t) by omega.
+    assert (hyp1: forall tc', tc' < t' -> ~ recv mch p c a tc' m') by (
+      unfold not; intros tc' tc'LtT' mrecvm'Tc';
+        pose proof (uniqRecv2 mrecvm' mrecvm'Tc'); intuition).
+    assert (hyp2: forall tp', tp' < t'' -> ~ recv mch c p a tp' m) by (
+      unfold not; intros tp' tp'LtT'' mrecvmTp';
+        pose proof (uniqRecv2 mrecvm mrecvmTp'); intuition).
+    pose proof (cross t' t'' t'LeT t''LeT m msendm m' msendm' hyp1 hyp2).
+    firstorder.
+    assert (noRecv': ~ (exists tc, S t' <= tc < tm /\ exists m, recv mch p c a tc m /\ to m >= state c a tm)) by
+      (
         unfold not; intros [tc [cond [m0 [mrecvm0 _]]]];
           assert (cond': t' < tc < tm) by omega; generalize noRecv cond' mrecvm0; clear; firstorder).
-      assert (nGt: ~ state c a tm > state c a (S t')) by (
-        assert (eqOrGt: tm = S t' \/ tm > S t') by omega;
-          destruct eqOrGt as [toEqSt' | toGtSt']; [
-            rewrite <- toEqSt';
-              omega |
-                pose proof (@whenChildHigh a (S t') tm toGtSt') as contra;
-                  generalize contra noRecv'; clear; firstorder]).
-      assert (dirEqSt: dir p c a (S ts) = state c a (S t')) by (
-        pose proof (sb.sendmChange msendm) as one;
-          pose proof (db.recvmChange mrecvm) as two;
-            unfold St.st, Dir.st in *;
-              congruence).
-      assert (stoLesSt': state c a tm <= state c a (S t')) by omega.
-      congruence.
-      pose proof (dirSendmImpRecvr msendm) as [r rrecvr].
-      pose proof (recvImpMarkSend rrecvr) as [t' [t'LeTs rsendr]].
-      destruct (classical (exists tc, tc < tm /\ recv mch p c a tc m)) as [[tc [tcLtTo mrecvm]] | notEx].
-      assert (eqOrNot: tm = S tc \/ tm > S tc) by omega.
-      destruct eqOrNot as [toEqStc | toGtStc].
-      assert (dirEqSt: state c a tm = dir p c a tm) by (
-        pose proof (db.sendmChange msendm) as one; pose proof (sb.recvmChange mrecvm) as two;
-          unfold St.st, Dir.st in *; congruence).
-      omega.
-      assert (noLower: ~ exists t'', S tc <= t'' < tm /\ exists m', recv mch p c a t'' m' /\ to m' >= state c a tm)
-        by (
+    assert (nGt: ~ state c a tm > state c a (S t')) by (
+      assert (eqOrGt: tm = S t' \/ tm > S t') by omega;
+        destruct eqOrGt as [toEqSt' | toGtSt']; [
+          rewrite <- toEqSt';
+            omega |
+              pose proof (@st.whenChildHigh a (S t') tm toGtSt') as contra;
+                generalize contra noRecv'; clear; firstorder]).
+    assert (dirEqSt: dir p c a (S ts) = state c a (S t')) by (
+      pose proof (st.sendmChange msendm) as one;
+        pose proof (dir.recvmChange mrecvm) as two;
+          unfold st.st, dir.st in *;
+            congruence).
+    assert (stoLesSt': state c a tm <= state c a (S t')) by omega.
+    congruence.
+    pose proof (dir.sendmImpRecvr msendm) as [r rrecvr].
+    pose proof (recvImpMarkSend rrecvr) as [t' [t'LeTs rsendr]].
+    destruct (classical (exists tc, tc < tm /\ recv mch p c a tc m)) as [[tc [tcLtTo mrecvm]] | notEx].
+    assert (eqOrNot: tm = S tc \/ tm > S tc) by omega.
+    destruct eqOrNot as [toEqStc | toGtStc].
+    assert (dirEqSt: state c a tm = dir p c a tm) by (
+      pose proof (dir.sendmChange msendm) as one; pose proof (st.recvmChange mrecvm) as two;
+        unfold st.st, dir.st in *; congruence).
+    omega.
+    assert (noLower: ~ exists t'', S tc <= t'' < tm /\ exists m', recv mch p c a t'' m' /\ to m' >= state c a tm)
+      by (
         unfold not; intros [t'' [cond [m' [mrecvm' _]]]];
           pose proof (recvImpMarkSend mrecvm') as [tf [tfLeT'' msendm']];
             assert (diff: ts = tf \/ tf < ts \/ tf > ts) by omega;
@@ -726,121 +781,121 @@ Module Type System (dataTypes: DataTypes) (ch: Channel dataTypes).
                                 apply (cReqPRespCross rsendr msendm' cross1 cross2)|
                                   assert (cond2: ts < tf < tm) by omega;
                                     generalize cond2 noPrevChnge msendm'; clear; firstorder]).
-      pose proof (@whenChildHigh a (S tc) tm toGtStc) as contra.
-      assert (not: ~ state c a tm > state c a (S tc)) by (generalize noLower contra; clear; firstorder).
-      assert (not2: state c a tm <= state c a (S tc)) by omega; clear not.
-      assert (dirEqSt: dir p c a (S ts) = state c a (S tc)) by (
-        pose proof (db.sendmChange msendm) as one; pose proof (sb.recvmChange mrecvm) as two;
-          unfold St.st, Dir.st in *; congruence).
-      omega.
-      assert (tsLeT: ts <= t) by omega.
-      assert (less: state c a ts <= dir p c a ts) by firstorder.
-      assert (tmGtTs: tm > t') by omega.
-      assert (noRecv: ~ exists t'', t' <= t'' < tm /\ exists m, recv mch p c a t'' m /\ to m >= state c a tm) by (
-        unfold not; intros [t'' [cond [m' [mrecvm' _]]]];
-          pose proof (recvImpMarkSend mrecvm') as [t1 [t1LeT'' msendm']];
-            assert (t1NeTs: t1 = ts -> False) by (
-              intros t1EqTs; rewrite t1EqTs in *;
-                pose proof (uniqMarksend1 msendm msendm') as mEqm';
-                  rewrite <- mEqm' in *; 
-                    generalize notEx cond mrecvm'; clear; firstorder);
-            assert (eqOrNot: t1 = ts \/ t1 > ts \/ t1 < ts) by omega;
-              destruct eqOrNot as [t1EqTs | [t1GtTs | t1LtTs]];
-                [firstorder |
-                  assert (cond2: ts < t1 < tm) by omega;
-                    generalize noPrevChnge cond2 msendm'; clear; firstorder |
-                      assert (one: forall tc', tc' < t' -> ~ recv mch p c a tc' m') by (
-                        unfold not; intros tc' tc'LtT' mrecvm'Tc';
-                          pose proof (uniqRecv2 mrecvm' mrecvm'Tc') as t''EqTc'; omega);
-                      assert (two: forall tp', tp' <= t1 -> ~ recv rch c p a tp' r) by (
-                        unfold not; intros tp' tp'LeT1 rrecvrTp';
-                          pose proof (uniqRecv2 rrecvr rrecvrTp') as tsEqTp'; omega);
-                      apply (cReqPRespCross rsendr msendm' one two)]).
-      assert (contra1: ~ state c a tm > state c a t') by (
-        unfold not; intros contra;
-          generalize (whenChildHigh tmGtTs contra) noRecv; clear; firstorder).
-      assert (cont: state c a tm <= state c a t') by omega.
-      pose proof (sb.sendrImpSt rsendr) as toRGtDir; unfold St.toRSComp in toRGtDir; unfold St.st in *.
-      pose proof (dirSendmImpRecvrGe msendm rrecvr) as toMGeToR.
-      pose proof (db.sendmChange msendm) as toMEq; unfold Dir.st in *.
-      omega.
-      assert (eqOrNot: 0 = tm \/ 0 < tm) by omega.
-      destruct eqOrNot as [tmEq0 | tmGt0].
-      rewrite <- tmEq0 in *; pose proof init as init; rewrite init in *; omega.
-      assert (premise: forall tn, 0 <= tn < tm -> (forall m, ~ Dir.mmarksend a tn m) /\
-        (forall m, ~ Dir.mrecv a tn m)) by (
+    pose proof (@st.whenChildHigh a (S tc) tm toGtStc) as contra.
+    assert (not: ~ state c a tm > state c a (S tc)) by (generalize noLower contra; clear; firstorder).
+    assert (not2: state c a tm <= state c a (S tc)) by omega; clear not.
+    assert (dirEqSt: dir p c a (S ts) = state c a (S tc)) by (
+      pose proof (dir.sendmChange msendm) as one; pose proof (st.recvmChange mrecvm) as two;
+        unfold st.st, dir.st in *; congruence).
+    omega.
+    assert (tsLeT: ts <= t) by omega.
+    assert (less: state c a ts <= dir p c a ts) by firstorder.
+    assert (tmGtTs: tm > t') by omega.
+    assert (noRecv: ~ exists t'', t' <= t'' < tm /\ exists m, recv mch p c a t'' m /\ to m >= state c a tm) by (
+      unfold not; intros [t'' [cond [m' [mrecvm' _]]]];
+        pose proof (recvImpMarkSend mrecvm') as [t1 [t1LeT'' msendm']];
+          assert (t1NeTs: t1 = ts -> False) by (
+            intros t1EqTs; rewrite t1EqTs in *;
+              pose proof (uniqMarksend1 msendm msendm') as mEqm';
+                rewrite <- mEqm' in *; 
+                  generalize notEx cond mrecvm'; clear; firstorder);
+          assert (eqOrNot: t1 = ts \/ t1 > ts \/ t1 < ts) by omega;
+            destruct eqOrNot as [t1EqTs | [t1GtTs | t1LtTs]];
+              [firstorder |
+                assert (cond2: ts < t1 < tm) by omega;
+                  generalize noPrevChnge cond2 msendm'; clear; firstorder |
+                    assert (one: forall tc', tc' < t' -> ~ recv mch p c a tc' m') by (
+                      unfold not; intros tc' tc'LtT' mrecvm'Tc';
+                        pose proof (uniqRecv2 mrecvm' mrecvm'Tc') as t''EqTc'; omega);
+                    assert (two: forall tp', tp' <= t1 -> ~ recv rch c p a tp' r) by (
+                      unfold not; intros tp' tp'LeT1 rrecvrTp';
+                        pose proof (uniqRecv2 rrecvr rrecvrTp') as tsEqTp'; omega);
+                    apply (cReqPRespCross rsendr msendm' one two)]).
+    assert (contra1: ~ state c a tm > state c a t') by (
+      unfold not; intros contra;
+        generalize (st.whenChildHigh tmGtTs contra) noRecv; clear; firstorder).
+    assert (cont: state c a tm <= state c a t') by omega.
+    pose proof (st.sendrImpSt rsendr) as toRGtDir; unfold st.toRSComp in toRGtDir; unfold st.st in *.
+    pose proof (dir.sendmImpRecvrGe msendm rrecvr) as toMGeToR.
+    pose proof (dir.sendmChange msendm) as toMEq; unfold dir.st in *.
+    omega.
+    assert (eqOrNot: 0 = tm \/ 0 < tm) by omega.
+    destruct eqOrNot as [tmEq0 | tmGt0].
+    rewrite <- tmEq0 in *; pose proof @init as init; rewrite init in *; omega.
+    assert (premise: forall tn, 0 <= tn < tm -> (forall m, ~ marksend mch p c a tn m) /\
+      (forall m, ~ recv mch c p a tn m)) by (
         intros tn [_ tnLtTm];
           constructor;
             unfold not; intros m msendm;
               generalize noChnge tnLtTm msendm; clear; firstorder).
-      pose proof (db.noChange tmGt0 premise) as dir0DirTm; unfold Dir.st in *.
-      pose proof @whenChildHigh.
-      assert (not: ~ exists t'', 0 <= t'' < tm /\ exists m, recv mch p c a t'' m /\ to m >= state c a tm) by (
-        unfold not; intros [t'' [[_ t''LtTm] [m [mrecvm _]]]];
-          pose proof (recvImpMarkSend mrecvm) as [t' [t'LeT'' msendm]];
-            assert (t'LtTm: t' < tm) by omega;
-              generalize noChnge t'LtTm msendm; clear; firstorder).
-      assert (done: ~ state c a tm > state c a 0) by (generalize (@whenChildHigh a 0 tm tmGt0) not;
-        clear; firstorder).
-      pose proof (init a) as start; omega.
+    pose proof (dir.noChange tmGt0 premise) as dir0DirTm; unfold dir.st in *.
+    pose proof @st.whenChildHigh.
+    assert (not: ~ exists t'', 0 <= t'' < tm /\ exists m, recv mch p c a t'' m /\ to m >= state c a tm) by (
+      unfold not; intros [t'' [[_ t''LtTm] [m [mrecvm _]]]];
+        pose proof (recvImpMarkSend mrecvm) as [t' [t'LeT'' msendm]];
+          assert (t'LtTm: t' < tm) by omega;
+            generalize noChnge t'LtTm msendm; clear; firstorder).
+    assert (done: ~ state c a tm > state c a 0) by (generalize (@st.whenChildHigh a 0 tm tmGt0) not;
+      clear; firstorder).
+    pose proof (@init a) as start; omega.
 
-      constructor.
-      apply cross'.
+    constructor.
+    apply cross'.
 
-      assert (cReqResp': forall {t1 t2 t3}, t3 <= S t -> forall {m}, marksend mch c p a t1 m -> forall {r},
-        marksend rch c p a t2 r -> recv rch c p a t3 r -> t1 <= t2 -> (forall t4, t4 < t3 -> ~ recv mch c p a t4 m) ->
-        False).
-      intros t1 t2 t3 t3LeSt m msendm r rsendr rrecvr t1LeT2 neg.
-      unfold Time in *.
-      assert (eqOrNot: t1 = t2 \/ t1 < t2) by omega.
-      destruct eqOrNot as [t1EqT2 | t1LtT2].
-      rewrite t1EqT2 in *.
-      pose proof (sb.noSendmSendr msendm rsendr); intuition.
-      clear t1LeT2.
-      pose proof (recvImpMarkSend rrecvr) as [t' [t'LeT3 rsend'r]].
-      pose proof (uniqMarksend2 rsendr rsend'r) as t2EqT'.
-      rewrite <- t2EqT' in *.
-      clear rsend'r t2EqT'.
-      assert (t1LeT: t1 <= t) by omega.
-      pose proof (cons t1 t1LeT) as st1Ledt1.
+    assert (cReqResp': forall {t1 t2 t3}, t3 <= S t -> forall {m}, marksend mch c p a t1 m -> forall {r},
+      marksend rch c p a t2 r -> recv rch c p a t3 r -> t1 <= t2 -> (forall t4, t4 < t3 -> ~ recv mch c p a t4 m) ->
+      False).
+    intros t1 t2 t3 t3LeSt m msendm r rsendr rrecvr t1LeT2 neg.
+    unfold Time in *.
+    assert (eqOrNot: t1 = t2 \/ t1 < t2) by omega.
+    destruct eqOrNot as [t1EqT2 | t1LtT2].
+    rewrite t1EqT2 in *.
+    pose proof (st.noSendmSendr msendm rsendr); intuition.
+    clear t1LeT2.
+    pose proof (recvImpMarkSend rrecvr) as [t' [t'LeT3 rsend'r]].
+    pose proof (uniqMarksend2 rsendr rsend'r) as t2EqT'.
+    rewrite <- t2EqT' in *.
+    clear rsend'r t2EqT'.
+    assert (t1LeT: t1 <= t) by omega.
+    pose proof (cons t1 t1LeT) as st1Ledt1.
 
-      assert (notty1: ~ exists t'', t1 <= t'' < t2 /\ exists m, recv mch p c a t'' m /\ to m >= state c a t2) by (
-        unfold not; intros [t'' [cond [m0 [mrecvm0 _]]]];
-          pose proof (recvImpMarkSend mrecvm0) as [t5 [t5LeT'' msendm0]];
-            assert (one: forall tc', tc' < t1 -> ~ recv mch p c a tc' m0) by (
-              unfold not; intros tc' tc'LtT1 mrecvM0Tc';
-                pose proof (uniqRecv2 mrecvm0 mrecvM0Tc') as t''EqTc';
-                  rewrite <- t''EqTc' in *; omega);
-            assert (two: forall tp', tp' < t5 -> ~ recv mch c p a tp' m) by (
-              unfold not; intros tp' tp'LtT5; assert (t5LtT3: tp' < t3) by omega; firstorder);
-            assert (t5Let: t5 <= t) by omega;
-              apply (cross t1 t5 t1LeT t5Let m msendm m0 msendm0 one two)).
-      assert (notty: ~ exists t'', S t1 <= t'' < t2 /\ exists m, recv mch p c a t'' m /\ to m >= state c a t2) by (
-        clear cRespResp;
-          unfold not; intros [t'' [cond ex]];
-            assert (cond2: t1 <= t'' < t2) by omega;
-              generalize notty1 cond2 ex; clear; firstorder).
-              
-      assert (notst2Gtst1: ~ state c a t2 > state c a (S t1)) by (
-        clear cRespResp;
+    assert (notty1: ~ exists t'', t1 <= t'' < t2 /\ exists m, recv mch p c a t'' m /\ to m >= state c a t2) by (
+      unfold not; intros [t'' [cond [m0 [mrecvm0 _]]]];
+        pose proof (recvImpMarkSend mrecvm0) as [t5 [t5LeT'' msendm0]];
+          assert (one: forall tc', tc' < t1 -> ~ recv mch p c a tc' m0) by (
+            unfold not; intros tc' tc'LtT1 mrecvM0Tc';
+              pose proof (uniqRecv2 mrecvm0 mrecvM0Tc') as t''EqTc';
+                rewrite <- t''EqTc' in *; omega);
+          assert (two: forall tp', tp' < t5 -> ~ recv mch c p a tp' m) by (
+            unfold not; intros tp' tp'LtT5; assert (t5LtT3: tp' < t3) by omega; firstorder);
+          assert (t5Let: t5 <= t) by omega;
+            apply (cross t1 t5 t1LeT t5Let m msendm m0 msendm0 one two)).
+    assert (notty: ~ exists t'', S t1 <= t'' < t2 /\ exists m, recv mch p c a t'' m /\ to m >= state c a t2) by (
+      clear cRespResp;
+        unfold not; intros [t'' [cond ex]];
+          assert (cond2: t1 <= t'' < t2) by omega;
+            generalize notty1 cond2 ex; clear; firstorder).
+    
+    assert (notst2Gtst1: ~ state c a t2 > state c a (S t1)) by (
+      clear cRespResp;
         clear notty1; assert (eqOrNot: S t1 = t2 \/ S t1 < t2) by omega;
           destruct eqOrNot as [eq| St1LtT2]; [
             rewrite eq;
               omega|
-                unfold not; intros st; pose proof (whenChildHigh St1LtT2 st) as some; firstorder]).
-      assert (stt2LestT1: state c a t2 <= state c a (S t1)) by omega.
-      pose proof (dirRecvrCond rrecvr) as fromRLe.
-      pose proof (sb.sendrFrom rsendr) as fromREq; unfold St.st in *.
-      pose proof (stSendmImpSt msendm) as stGt.
-      pose proof (sb.sendmChange msendm) as stEq; unfold St.st in *.
-      rewrite fromREq, <- stEq in *.
-      assert (drGt: dir p c a t1 > dir p c a t3) by omega.
-      assert (drNe: dir p c a t1 <> dir p c a t3) by omega.
-      assert (sendRecv: ~ forall tn, t1 <= tn < t3 -> (forall m, ~ marksend mch p c a tn m) /\
-        (forall m, ~ recv mch c p a tn m)) by (
-        unfold not; intros exp; assert (t1LtT3: t1 < t3) by omega; pose proof (db.noChange t1LtT3 exp); firstorder).
-      assert (noSend: forall tn, t1 <= tn < t3 -> forall m, ~ marksend mch p c a tn m) by (
-        clear cRespResp;
+                unfold not; intros st; pose proof (st.whenChildHigh St1LtT2 st) as some; firstorder]).
+    assert (stt2LestT1: state c a t2 <= state c a (S t1)) by omega.
+    pose proof (dir.recvrCond rrecvr) as fromRLe.
+    pose proof (st.sendrFrom rsendr) as fromREq; unfold st.st in *.
+    pose proof (st.sendmImpSt msendm) as stGt.
+    pose proof (st.sendmChange msendm) as stEq; unfold st.st in *.
+    rewrite fromREq, <- stEq in *.
+    assert (drGt: dir p c a t1 > dir p c a t3) by omega.
+    assert (drNe: dir p c a t1 <> dir p c a t3) by omega.
+    assert (sendRecv: ~ forall tn, t1 <= tn < t3 -> (forall m, ~ marksend mch p c a tn m) /\
+      (forall m, ~ recv mch c p a tn m)) by (
+        unfold not; intros exp; assert (t1LtT3: t1 < t3) by omega; pose proof (dir.noChange t1LtT3 exp); firstorder).
+    assert (noSend: forall tn, t1 <= tn < t3 -> forall m, ~ marksend mch p c a tn m) by (
+      clear cRespResp;
         unfold not; intros tn cond m0 msendm0;
           assert (tnLeT: tn <= t) by omega;
             assert (one: forall tc', tc' < t1 -> ~ recv mch p c a tc' m0) by (
@@ -852,223 +907,223 @@ Module Type System (dataTypes: DataTypes) (ch: Channel dataTypes).
               unfold not; intros tp' tp'LtTn; assert (tp'LtT3: tp' < t3) by omega; firstorder);
             apply (cross t1 tn t1LeT tnLeT m msendm m0 msendm0 one two)).
 
-      destruct (classical (exists tn, tn < t3 /\ t1 <= tn /\ exists m0, recv mch c p a tn m0)) as [ext|noEx].
-      pose proof (maxExists' classical ext) as [tn [cond [[tnLtT3 [m0 mrecvm0]] notAfter]]].
-      
-      pose proof (recvImpMarkSend mrecvm0) as [tr [trLeTn msendm0]].
-      assert (opts: tr = t1 \/ tr > t1 \/ tr < t1) by omega.
-      destruct opts as [trEqT1 | [trGtT1 | trLtT1]].
-      rewrite trEqT1 in *.
-      pose proof (uniqMarksend1 msendm msendm0) as mEqm0.
-      rewrite <- mEqm0 in *.
-      generalize neg cond mrecvm0; clear; firstorder.
-      assert (tnLeT: tn <= t) by omega.
-      assert (cond2: forall t4, t4 < tn -> ~ recv mch c p a t4 m) by (
-        intros t4 t4LtTn; assert (t4LtT3: t4 < t3) by omega;
-          generalize neg t4LtT3; clear; firstorder).
-      apply (cRespResp t1 tr tn tnLeT m msendm m0 msendm0 mrecvm0 trGtT1 cond2).
-      assert (notty2': ~ exists t'', tr <= t'' < t1 /\ exists m, recv mch p c a t'' m /\ to m >= state c a t1) by (
-        unfold not; intros [t'' [cond2 [m1 [mrecvm1 _]]]];
-          pose proof (recvImpMarkSend mrecvm1) as [t5 [t5LeT'' msendm1]];
-            assert (trLeT: tr <= t) by omega;
-              assert (t5LeT: t5 <= t) by omega;
-                assert (one: forall tc', tc' < tr -> ~ recv mch p c a tc' m1) by (
-                  unfold not; intros tc' tc'LtTr mrecv'm1;
-                    pose proof (uniqRecv2 mrecvm1 mrecv'm1) as t''EqTc';
-                      rewrite <- t''EqTc' in *;
-                        omega);
-                assert (two: forall tp', tp' < t5 -> ~ recv mch c p a tp' m0) by (
-                  unfold not; intros tp' tp'LtT5 mrecv'm0;
-                    pose proof (uniqRecv2 mrecvm0 mrecv'm0) as tnEqTp';
-                      rewrite <- tnEqTp' in *; omega);
-                apply (cross tr t5 trLeT t5LeT m0 msendm0 m1 msendm1 one two)).
-      assert (notty2: ~ exists t'', S tr <= t'' < t1 /\ exists m, recv mch p c a t'' m /\ to m >= state c a t1) by (
-        unfold not; intros [t'' [cond1 rest]]; assert (cond2: tr <= t'' < t1) by omega;
-          generalize notty2' cond2 rest; clear; firstorder).
-      assert (strLeT1: S tr <= t1) by omega.
-      pose proof (whenChildHighConv strLeT1 notty2) as st1LeTr.
-      pose proof (whenChildHighConv t1LtT2 notty) as sST1LeT2.
-      assert (trLtT3: tr < t3) by omega.
-      assert (noC: forall tn0, S tn <= tn0 < t3 -> (forall m, ~ marksend mch p c a tn0 m) /\
-        (forall m, ~ recv mch c p a tn0 m)) by (
+    destruct (classical (exists tn, tn < t3 /\ t1 <= tn /\ exists m0, recv mch c p a tn m0)) as [ext|noEx].
+    pose proof (maxExists' classical ext) as [tn [cond [[tnLtT3 [m0 mrecvm0]] notAfter]]].
+    
+    pose proof (recvImpMarkSend mrecvm0) as [tr [trLeTn msendm0]].
+    assert (opts: tr = t1 \/ tr > t1 \/ tr < t1) by omega.
+    destruct opts as [trEqT1 | [trGtT1 | trLtT1]].
+    rewrite trEqT1 in *.
+    pose proof (uniqMarksend1 msendm msendm0) as mEqm0.
+    rewrite <- mEqm0 in *.
+    generalize neg cond mrecvm0; clear; firstorder.
+    assert (tnLeT: tn <= t) by omega.
+    assert (cond2: forall t4, t4 < tn -> ~ recv mch c p a t4 m) by (
+      intros t4 t4LtTn; assert (t4LtT3: t4 < t3) by omega;
+        generalize neg t4LtT3; clear; firstorder).
+    apply (cRespResp t1 tr tn tnLeT m msendm m0 msendm0 mrecvm0 trGtT1 cond2).
+    assert (notty2': ~ exists t'', tr <= t'' < t1 /\ exists m, recv mch p c a t'' m /\ to m >= state c a t1) by (
+      unfold not; intros [t'' [cond2 [m1 [mrecvm1 _]]]];
+        pose proof (recvImpMarkSend mrecvm1) as [t5 [t5LeT'' msendm1]];
+          assert (trLeT: tr <= t) by omega;
+            assert (t5LeT: t5 <= t) by omega;
+              assert (one: forall tc', tc' < tr -> ~ recv mch p c a tc' m1) by (
+                unfold not; intros tc' tc'LtTr mrecv'm1;
+                  pose proof (uniqRecv2 mrecvm1 mrecv'm1) as t''EqTc';
+                    rewrite <- t''EqTc' in *;
+                      omega);
+              assert (two: forall tp', tp' < t5 -> ~ recv mch c p a tp' m0) by (
+                unfold not; intros tp' tp'LtT5 mrecv'm0;
+                  pose proof (uniqRecv2 mrecvm0 mrecv'm0) as tnEqTp';
+                    rewrite <- tnEqTp' in *; omega);
+              apply (cross tr t5 trLeT t5LeT m0 msendm0 m1 msendm1 one two)).
+    assert (notty2: ~ exists t'', S tr <= t'' < t1 /\ exists m, recv mch p c a t'' m /\ to m >= state c a t1) by (
+      unfold not; intros [t'' [cond1 rest]]; assert (cond2: tr <= t'' < t1) by omega;
+        generalize notty2' cond2 rest; clear; firstorder).
+    assert (strLeT1: S tr <= t1) by omega.
+    pose proof (st.whenChildHighConv strLeT1 notty2) as st1LeTr.
+    pose proof (st.whenChildHighConv t1LtT2 notty) as sST1LeT2.
+    assert (trLtT3: tr < t3) by omega.
+    assert (noC: forall tn0, S tn <= tn0 < t3 -> (forall m, ~ marksend mch p c a tn0 m) /\
+      (forall m, ~ recv mch c p a tn0 m)) by (
         intros tn0 cond2;
           constructor; [assert (cond3: t1 <= tn0 < t3) by omega; generalize noSend cond3; clear; firstorder|
             assert (cond4: tn < tn0 < t3) by omega; 
               assert (t1LeTn0: t1 <= tn0) by omega; generalize cond4 t1LeTn0 notAfter; clear; firstorder]).
-      assert (sTnLtT3: S tn <= t3) by omega.
-      pose proof (db.noChange2 sTnLtT3 noC) as dirEq.
-      unfold Dir.st in *.
-      generalize st1LeTr sST1LeT2 sTnLtT3 dirEq rsendr rrecvr msendm msendm0 mrecvm0; clear; intros.
-      pose proof (sb.sendmChange msendm) as sEqTom.
-      pose proof (stSendmImpSt msendm) as sGtTom.
-      pose proof (db.recvmChange mrecvm0) as dSEqTom0.
-      pose proof (sb.sendmChange msendm0) as sSEqTom0.
-      pose proof (dirRecvrCond rrecvr) as dLeFromr.
-      pose proof (sb.sendrFrom rsendr) as sEqFromr.
-      unfold St.st, Dir.st in *. omega.
-      generalize sendRecv noSend noEx; clear; firstorder.
+    assert (sTnLtT3: S tn <= t3) by omega.
+    pose proof (dir.noChange2 sTnLtT3 noC) as dirEq.
+    unfold dir.st in *.
+    generalize st1LeTr sST1LeT2 sTnLtT3 dirEq rsendr rrecvr msendm msendm0 mrecvm0; clear; intros.
+    pose proof (st.sendmChange msendm) as sEqTom.
+    pose proof (st.sendmImpSt msendm) as sGtTom.
+    pose proof (dir.recvmChange mrecvm0) as dSEqTom0.
+    pose proof (st.sendmChange msendm0) as sSEqTom0.
+    pose proof (dir.recvrCond rrecvr) as dLeFromr.
+    pose proof (st.sendrFrom rsendr) as sEqFromr.
+    unfold st.st, dir.st in *. omega.
+    generalize sendRecv noSend noEx; clear; firstorder.
 
-      constructor.
+    constructor.
 
-      intros tc tp tcLeSt tpLeSt mc msendmc mp msendmp norecvmp norecvmc.
-      pose proof (dirSendmImpRecvr msendmp) as [r rrecvr].
-      pose proof (recvImpMarkSend rrecvr) as [t1 [t1LeTp rsendr]].
-      assert (opts: t1 = tc \/ tc < t1 \/ t1 < tc) by omega.
-      destruct opts as [t1EqTc | [tcLtT1 | t1LtTc]].
-      rewrite t1EqTc in *.
-      apply (sb.noSendmSendr msendmc rsendr).
-      assert (tcLeT1: tc <= t1) by omega.
-      apply (cReqResp' tc t1 tp tpLeSt mc msendmc r rsendr rrecvr tcLeT1 norecvmc).
-      destruct (classical (exists tm, t1 <= tm < tc /\ exists m, recv mch p c a tm m)) as [ext|noExt].
-      destruct ext as [tm [[t1LeTm tmLtTc] [m recvm]]].
-      pose proof (recvImpMarkSend recvm) as [tn [tnLeTm sendm]].
-      assert (opts: tn = tp \/ tn < tp \/ tn > tp) by omega.
-      destruct opts as [tnEqTp | [tnLtTp | tnGtTp]].
-      rewrite tnEqTp in *.
-      pose proof (uniqMarksend1 sendm msendmp) as mEqMp.
-      rewrite mEqMp in *.
-      firstorder.
-      assert (one: forall tc', tc' < t1 -> ~ recv mch p c a tc' m) by (
-        unfold not; intros tc' tc'LtT1 recv'm;
-          pose proof (uniqRecv2 recvm recv'm) as tmEqTc';
-            omega).
-      assert (two: forall tp', tp' <= tn -> ~ recv rch c p a tp' r) by (
-        unfold not; intros tp' tp'LeTn recv'r;
-          pose proof (uniqRecv2 rrecvr recv'r) as tpEqTp';
-            omega).
-      apply (cReqPRespCross rsendr sendm one two).
-      pose proof (dirSendmImpRecvr sendm) as [r1 recvr1].
-      pose proof (recvImpMarkSend recvr1) as [tq [tqLeTn sendr1]].
-      assert (one: forall tc', tc' < tq -> ~ recv mch p c a tc' mp) by (
-        unfold not; intros tc' tc'LtTq; assert (tc'LtTc: tc' < tc) by omega;
-          apply (norecvmp tc' tc'LtTc)).
-      assert (two: forall tp', tp' <= tp -> ~ recv rch c p a tp' r1) by (
-        unfold not; intros tp' tp'LeTp recv'r1;
-          pose proof (uniqRecv2 recvr1 recv'r1) as tpEqTp';
-            omega).
-      apply (cReqPRespCross sendr1 msendmp one two).
-      assert (opt: ~ exists tm, t1 <= tm < tc /\ exists m, recv mch p c a tm m) by (
-        generalize noExt; clear; firstorder).
-      assert (opt': forall t', t1 < t' <= tc -> ~ exists tm, t1 <= tm < t' /\ exists m,
-        recv mch p c a tm m /\ to m >= state c a t') by (
-          unfold not; intros t' t'LtTc [tm [cond rest]]; assert (cond2: t1 <= tm < tc) by omega;
-            generalize opt t'LtTc cond2 rest; clear; firstorder).
-      assert (notSth: forall t', t1 < t' <= tc -> ~ state c a t' > state c a t1) by (
-        unfold not; intros t' [t1LtT' t'LeTc] sgt;
-          pose proof (whenChildHigh t1LtT' sgt) as contra;
-            generalize opt' contra t1LtT' t'LeTc; clear; firstorder).
-      assert (stcLet1: forall t', t1 < t' <= tc -> state c a t' <= state c a t1) by (intros t' cond;
-        specialize (notSth t' cond); omega).
-      clear notSth opt opt'.
-      pose proof (sb.sendrImpSt rsendr) as gtRel.
-      unfold St.toRSComp, St.st in *.
-      assert (stcLet2: forall t', t1 < t' <= tc -> state c a t' < to r) by (
-        intros t' cond; specialize (stcLet1 t' cond); omega).
-      clear stcLet1 gtRel.
-      pose proof (stVoluntary rsendr t1LtTc msendmc stcLet2) as [r1 recvr1].
-      pose proof (recvImpMarkSend recvr1) as [t2 [t2LeT1 sendr1]].
-      assert (t2LeTp: t2 = tp \/ t2 > tp \/ t2 < tp) by omega.
-      destruct t2LeTp as [t2EqTp | [t2GtTp | t2LtTp]].
-      rewrite t2EqTp in *.
-      apply (db.noSendmSendr msendmp sendr1).
-      assert (tpLeT2: tp <= t2) by omega.
-      pose proof (pRespReq noTwoPResp noTwoPReqNon msendmp sendr1 recvr1 tpLeT2) as [t4 [t4LtTp recvmp]].
-      generalize norecvmp recvmp t4LtTp; clear; firstorder.
-      pose proof (dirSendrImpNoSendm t2LtTp sendr1 msendmp) as [t' [[t2LtT' t'LtTp] [m [recvm toMGeToR1]]]].
-      pose proof (recvImpMarkSend recvm) as [t'' [t''LeT' sendm]].
-      pose proof (sb.sendmChange sendm) as stEqToM. unfold St.st in *.
-      pose proof (stRecvrNoSendm recvr1 msendmc) as sTcGtToR1.
-      assert (stTcGtStST'': state c a tc > state c a (S t'')) by omega.
-      assert (opts: t'' = tc \/ t'' > tc \/ t'' < tc) by omega.
-      destruct opts as [t''EqTc | [t''GtTc | t''LtTc]].
-      rewrite t''EqTc in *.
-      pose proof (uniqMarksend1 msendmc sendm) as mEqMc.
-      rewrite mEqMc in *.
-      generalize t'LtTp recvm norecvmc; clear; firstorder.
-      assert (t'Let: t' <= t) by omega.
-      assert (norecv: forall t4, t4 < t' -> ~ recv mch c p a t4 mc) by (
-        unfold not; intros t4 t4LtT'; assert (t4LtTp: t4 < tp) by omega;
-          generalize norecvmc t4LtTp; clear; firstorder).
-      apply (cRespResp tc t'' t' t'Let mc msendmc m sendm recvm t''GtTc); intuition.
-      assert (opts: S t'' = tc \/ S t'' < tc) by omega.
-      destruct opts as [St''EqTc | St''LtTc].
-      rewrite St''EqTc in *.
-      omega.
-      pose proof (whenChildHigh St''LtTc stTcGtStST'') as [ts [cond [s [recvs _]]]].
-      pose proof (recvImpMarkSend recvs) as [tsr [tsrLeTs sends]].
-      assert (opts: tsr = t' \/ tsr > t' \/ tsr < t') by omega.
-      destruct opts as [tsrEqT' | [tsrGtT' | tsrLtT']].
-      rewrite tsrEqT' in *.
-      apply (db.noSendmRecvm sends recvm).
-      assert (t2LeTsr: t2 <= tsr) by omega.
-      pose proof (pReqResp noTwoPResp noTwoPReqNon sendr1 sends recvs t2LeTsr) as [tf [tfLtTs recv'r1]].
-      assert (tfLtTc: tf < tc) by omega.
-      pose proof (uniqRecv2 recvr1 recv'r1) as tcEqTf.
-      omega.
-      assert (t''LeT: t'' <= t) by omega.
-      assert (tsrLeT: tsr <= t) by omega.
-      assert (one: forall tc', tc' < t'' -> ~ recv mch p c a tc' s) by (
-        unfold not; intros tc' tc'LtT'' recv's; pose proof (uniqRecv2 recvs recv's) as tc'EqT';
-          rewrite tc'EqT' in *; omega).
-      assert (two: forall tp', tp' < tsr -> ~ recv mch c p a tp' m) by (
-        unfold not; intros tp' tp'LtTsr recv'm; pose proof (uniqRecv2 recvm recv'm) as tp'EqTsr;
+    intros tc tp tcLeSt tpLeSt mc msendmc mp msendmp norecvmp norecvmc.
+    pose proof (dir.sendmImpRecvr msendmp) as [r rrecvr].
+    pose proof (recvImpMarkSend rrecvr) as [t1 [t1LeTp rsendr]].
+    assert (opts: t1 = tc \/ tc < t1 \/ t1 < tc) by omega.
+    destruct opts as [t1EqTc | [tcLtT1 | t1LtTc]].
+    rewrite t1EqTc in *.
+    apply (st.noSendmSendr msendmc rsendr).
+    assert (tcLeT1: tc <= t1) by omega.
+    apply (cReqResp' tc t1 tp tpLeSt mc msendmc r rsendr rrecvr tcLeT1 norecvmc).
+    destruct (classical (exists tm, t1 <= tm < tc /\ exists m, recv mch p c a tm m)) as [ext|noExt].
+    destruct ext as [tm [[t1LeTm tmLtTc] [m recvm]]].
+    pose proof (recvImpMarkSend recvm) as [tn [tnLeTm sendm]].
+    assert (opts: tn = tp \/ tn < tp \/ tn > tp) by omega.
+    destruct opts as [tnEqTp | [tnLtTp | tnGtTp]].
+    rewrite tnEqTp in *.
+    pose proof (uniqMarksend1 sendm msendmp) as mEqMp.
+    rewrite mEqMp in *.
+    firstorder.
+    assert (one: forall tc', tc' < t1 -> ~ recv mch p c a tc' m) by (
+      unfold not; intros tc' tc'LtT1 recv'm;
+        pose proof (uniqRecv2 recvm recv'm) as tmEqTc';
           omega).
-      apply (cross t'' tsr t''LeT tsrLeT  m sendm s sends one two).
+    assert (two: forall tp', tp' <= tn -> ~ recv rch c p a tp' r) by (
+      unfold not; intros tp' tp'LeTn recv'r;
+        pose proof (uniqRecv2 rrecvr recv'r) as tpEqTp';
+          omega).
+    apply (cReqPRespCross rsendr sendm one two).
+    pose proof (dir.sendmImpRecvr sendm) as [r1 recvr1].
+    pose proof (recvImpMarkSend recvr1) as [tq [tqLeTn sendr1]].
+    assert (one: forall tc', tc' < tq -> ~ recv mch p c a tc' mp) by (
+      unfold not; intros tc' tc'LtTq; assert (tc'LtTc: tc' < tc) by omega;
+        apply (norecvmp tc' tc'LtTc)).
+    assert (two: forall tp', tp' <= tp -> ~ recv rch c p a tp' r1) by (
+      unfold not; intros tp' tp'LeTp recv'r1;
+        pose proof (uniqRecv2 recvr1 recv'r1) as tpEqTp';
+          omega).
+    apply (cReqPRespCross sendr1 msendmp one two).
+    assert (opt: ~ exists tm, t1 <= tm < tc /\ exists m, recv mch p c a tm m) by (
+      generalize noExt; clear; firstorder).
+    assert (opt': forall t', t1 < t' <= tc -> ~ exists tm, t1 <= tm < t' /\ exists m,
+      recv mch p c a tm m /\ to m >= state c a t') by (
+        unfold not; intros t' t'LtTc [tm [cond rest]]; assert (cond2: t1 <= tm < tc) by omega;
+          generalize opt t'LtTc cond2 rest; clear; firstorder).
+    assert (notSth: forall t', t1 < t' <= tc -> ~ state c a t' > state c a t1) by (
+      unfold not; intros t' [t1LtT' t'LeTc] sgt;
+        pose proof (st.whenChildHigh t1LtT' sgt) as contra;
+          generalize opt' contra t1LtT' t'LeTc; clear; firstorder).
+    assert (stcLet1: forall t', t1 < t' <= tc -> state c a t' <= state c a t1) by (intros t' cond;
+      specialize (notSth t' cond); omega).
+    clear notSth opt opt'.
+    pose proof (st.sendrImpSt rsendr) as gtRel.
+    unfold st.toRSComp, st.st in *.
+    assert (stcLet2: forall t', t1 < t' <= tc -> state c a t' < to r) by (
+      intros t' cond; specialize (stcLet1 t' cond); omega).
+    clear stcLet1 gtRel.
+    pose proof (st.voluntary rsendr t1LtTc msendmc stcLet2) as [r1 recvr1].
+    pose proof (recvImpMarkSend recvr1) as [t2 [t2LeT1 sendr1]].
+    assert (t2LeTp: t2 = tp \/ t2 > tp \/ t2 < tp) by omega.
+    destruct t2LeTp as [t2EqTp | [t2GtTp | t2LtTp]].
+    rewrite t2EqTp in *.
+    apply (dir.noSendmSendr msendmp sendr1).
+    assert (tpLeT2: tp <= t2) by omega.
+    pose proof (pRespReq noTwoPResp noTwoPReqNon msendmp sendr1 recvr1 tpLeT2) as [t4 [t4LtTp recvmp]].
+    generalize norecvmp recvmp t4LtTp; clear; firstorder.
+    pose proof (dir.sendrImpNoSendm t2LtTp sendr1 msendmp) as [t' [[t2LtT' t'LtTp] [m [recvm toMGeToR1]]]].
+    pose proof (recvImpMarkSend recvm) as [t'' [t''LeT' sendm]].
+    pose proof (st.sendmChange sendm) as stEqToM. unfold st.st in *.
+    pose proof (st.recvrNoSendm recvr1 msendmc) as sTcGtToR1.
+    assert (stTcGtStST'': state c a tc > state c a (S t'')) by omega.
+    assert (opts: t'' = tc \/ t'' > tc \/ t'' < tc) by omega.
+    destruct opts as [t''EqTc | [t''GtTc | t''LtTc]].
+    rewrite t''EqTc in *.
+    pose proof (uniqMarksend1 msendmc sendm) as mEqMc.
+    rewrite mEqMc in *.
+    generalize t'LtTp recvm norecvmc; clear; firstorder.
+    assert (t'Let: t' <= t) by omega.
+    assert (norecv: forall t4, t4 < t' -> ~ recv mch c p a t4 mc) by (
+      unfold not; intros t4 t4LtT'; assert (t4LtTp: t4 < tp) by omega;
+        generalize norecvmc t4LtTp; clear; firstorder).
+    apply (cRespResp tc t'' t' t'Let mc msendmc m sendm recvm t''GtTc); intuition.
+    assert (opts: S t'' = tc \/ S t'' < tc) by omega.
+    destruct opts as [St''EqTc | St''LtTc].
+    rewrite St''EqTc in *.
+    omega.
+    pose proof (st.whenChildHigh St''LtTc stTcGtStST'') as [ts [cond [s [recvs _]]]].
+    pose proof (recvImpMarkSend recvs) as [tsr [tsrLeTs sends]].
+    assert (opts: tsr = t' \/ tsr > t' \/ tsr < t') by omega.
+    destruct opts as [tsrEqT' | [tsrGtT' | tsrLtT']].
+    rewrite tsrEqT' in *.
+    apply (dir.noSendmRecvm sends recvm).
+    assert (t2LeTsr: t2 <= tsr) by omega.
+    pose proof (pReqResp noTwoPResp noTwoPReqNon sendr1 sends recvs t2LeTsr) as [tf [tfLtTs recv'r1]].
+    assert (tfLtTc: tf < tc) by omega.
+    pose proof (uniqRecv2 recvr1 recv'r1) as tcEqTf.
+    omega.
+    assert (t''LeT: t'' <= t) by omega.
+    assert (tsrLeT: tsr <= t) by omega.
+    assert (one: forall tc', tc' < t'' -> ~ recv mch p c a tc' s) by (
+      unfold not; intros tc' tc'LtT'' recv's; pose proof (uniqRecv2 recvs recv's) as tc'EqT';
+        rewrite tc'EqT' in *; omega).
+    assert (two: forall tp', tp' < tsr -> ~ recv mch c p a tp' m) by (
+      unfold not; intros tp' tp'LtTsr recv'm; pose proof (uniqRecv2 recvm recv'm) as tp'EqTsr;
+        omega).
+    apply (cross t'' tsr t''LeT tsrLeT  m sendm s sends one two).
 
-      constructor.
-      intuition.
+    constructor.
+    intuition.
 
-      intros t1 t2 t3 t3LeSt m msendm r rsendr rrecvr t1LeT2 neg.
-      unfold Time in *.
-      assert (eqOrNot: t1 = t2 \/ t1 < t2) by omega.
-      destruct eqOrNot as [t1EqT2 | t1LtT2].
-      rewrite t1EqT2 in *.
-      pose proof (uniqMarksend1 msendm rsendr) as mEqR; omega.
-      clear t1LeT2.
-      pose proof (recvImpMarkSend rrecvr) as [t' [t'LeT3 rsend'r]].
-      pose proof (uniqMarksend2 rsendr rsend'r) as t2EqT'.
-      rewrite <- t2EqT' in *.
-      clear rsend'r t2EqT'.
-      assert (t1LeT: t1 <= t) by omega.
-      pose proof (cons t1 t1LeT) as st1Ledt1.
+    intros t1 t2 t3 t3LeSt m msendm r rsendr rrecvr t1LeT2 neg.
+    unfold Time in *.
+    assert (eqOrNot: t1 = t2 \/ t1 < t2) by omega.
+    destruct eqOrNot as [t1EqT2 | t1LtT2].
+    rewrite t1EqT2 in *.
+    pose proof (uniqMarksend1 msendm rsendr) as mEqR; omega.
+    clear t1LeT2.
+    pose proof (recvImpMarkSend rrecvr) as [t' [t'LeT3 rsend'r]].
+    pose proof (uniqMarksend2 rsendr rsend'r) as t2EqT'.
+    rewrite <- t2EqT' in *.
+    clear rsend'r t2EqT'.
+    assert (t1LeT: t1 <= t) by omega.
+    pose proof (cons t1 t1LeT) as st1Ledt1.
 
-      assert (notty1: ~ exists t'', t1 <= t'' < t2 /\ exists m, recv mch p c a t'' m /\ to m >= state c a t2) by (
-        unfold not; intros [t'' [cond [m0 [mrecvm0 _]]]];
-          pose proof (recvImpMarkSend mrecvm0) as [t5 [t5LeT'' msendm0]];
-            assert (one: forall tc', tc' < t1 -> ~ recv mch p c a tc' m0) by (
-              unfold not; intros tc' tc'LtT1 mrecvM0Tc';
-                pose proof (uniqRecv2 mrecvm0 mrecvM0Tc') as t''EqTc';
-                  rewrite <- t''EqTc' in *; omega);
-            assert (two: forall tp', tp' < t5 -> ~ recv mch c p a tp' m) by (
-              unfold not; intros tp' tp'LtT5; assert (t5LtT3: tp' < t3) by omega; firstorder);
-            assert (t5Let: t5 <= t) by omega;
-              apply (cross t1 t5 t1LeT t5Let m msendm m0 msendm0 one two)).
-      assert (notty: ~ exists t'', S t1 <= t'' < t2 /\ exists m, recv mch p c a t'' m /\ to m >= state c a t2) by (
-        clear cRespResp;
-          unfold not; intros [t'' [cond ex]];
-            assert (cond2: t1 <= t'' < t2) by omega;
-              generalize notty1 cond2 ex; clear; firstorder).
-              
-      assert (notst2Gtst1: ~ state c a t2 > state c a (S t1)) by (
-        clear cRespResp;
+    assert (notty1: ~ exists t'', t1 <= t'' < t2 /\ exists m, recv mch p c a t'' m /\ to m >= state c a t2) by (
+      unfold not; intros [t'' [cond [m0 [mrecvm0 _]]]];
+        pose proof (recvImpMarkSend mrecvm0) as [t5 [t5LeT'' msendm0]];
+          assert (one: forall tc', tc' < t1 -> ~ recv mch p c a tc' m0) by (
+            unfold not; intros tc' tc'LtT1 mrecvM0Tc';
+              pose proof (uniqRecv2 mrecvm0 mrecvM0Tc') as t''EqTc';
+                rewrite <- t''EqTc' in *; omega);
+          assert (two: forall tp', tp' < t5 -> ~ recv mch c p a tp' m) by (
+            unfold not; intros tp' tp'LtT5; assert (t5LtT3: tp' < t3) by omega; firstorder);
+          assert (t5Let: t5 <= t) by omega;
+            apply (cross t1 t5 t1LeT t5Let m msendm m0 msendm0 one two)).
+    assert (notty: ~ exists t'', S t1 <= t'' < t2 /\ exists m, recv mch p c a t'' m /\ to m >= state c a t2) by (
+      clear cRespResp;
+        unfold not; intros [t'' [cond ex]];
+          assert (cond2: t1 <= t'' < t2) by omega;
+            generalize notty1 cond2 ex; clear; firstorder).
+    
+    assert (notst2Gtst1: ~ state c a t2 > state c a (S t1)) by (
+      clear cRespResp;
         clear notty1; assert (eqOrNot: S t1 = t2 \/ S t1 < t2) by omega;
           destruct eqOrNot as [eq| St1LtT2]; [
             rewrite eq;
               omega|
-                unfold not; intros st; pose proof (whenChildHigh St1LtT2 st) as some; firstorder]).
-      assert (stt2LestT1: state c a t2 <= state c a (S t1)) by omega.
-      pose proof (dirRecvmCond rrecvr) as fromRLe.
-      pose proof (sb.sendmFrom rsendr) as fromREq; unfold St.st in *.
-      pose proof (stSendmImpSt msendm) as stGt.
-      pose proof (sb.sendmChange msendm) as stEq; unfold St.st in *.
-      rewrite fromREq, <- stEq in *.
-      assert (drGt: dir p c a t1 > dir p c a t3) by omega.
-      assert (drNe: dir p c a t1 <> dir p c a t3) by omega.
-      assert (sendRecv: ~ forall tn, t1 <= tn < t3 -> (forall m, ~ marksend mch p c a tn m) /\
-        (forall m, ~ recv mch c p a tn m)) by (
-        unfold not; intros exp; assert (t1LtT3: t1 < t3) by omega; pose proof (db.noChange t1LtT3 exp); firstorder).
-      assert (noSend: forall tn, t1 <= tn < t3 -> forall m, ~ marksend mch p c a tn m) by (
-        clear cRespResp;
+                unfold not; intros st; pose proof (st.whenChildHigh St1LtT2 st) as some; firstorder]).
+    assert (stt2LestT1: state c a t2 <= state c a (S t1)) by omega.
+    pose proof (dir.recvmCond rrecvr) as fromRLe.
+    pose proof (st.sendmFrom rsendr) as fromREq; unfold st.st in *.
+    pose proof (st.sendmImpSt msendm) as stGt.
+    pose proof (st.sendmChange msendm) as stEq; unfold st.st in *.
+    rewrite fromREq, <- stEq in *.
+    assert (drGt: dir p c a t1 > dir p c a t3) by omega.
+    assert (drNe: dir p c a t1 <> dir p c a t3) by omega.
+    assert (sendRecv: ~ forall tn, t1 <= tn < t3 -> (forall m, ~ marksend mch p c a tn m) /\
+      (forall m, ~ recv mch c p a tn m)) by (
+        unfold not; intros exp; assert (t1LtT3: t1 < t3) by omega; pose proof (dir.noChange t1LtT3 exp); firstorder).
+    assert (noSend: forall tn, t1 <= tn < t3 -> forall m, ~ marksend mch p c a tn m) by (
+      clear cRespResp;
         unfold not; intros tn cond m0 msendm0;
           assert (tnLeT: tn <= t) by omega;
             assert (one: forall tc', tc' < t1 -> ~ recv mch p c a tc' m0) by (
@@ -1080,277 +1135,275 @@ Module Type System (dataTypes: DataTypes) (ch: Channel dataTypes).
               unfold not; intros tp' tp'LtTn; assert (tp'LtT3: tp' < t3) by omega; firstorder);
             apply (cross t1 tn t1LeT tnLeT m msendm m0 msendm0 one two)).
 
-      destruct (classical (exists tn, tn < t3 /\ t1 <= tn /\ exists m0, recv mch c p a tn m0)) as [ext|noEx].
-      pose proof (maxExists' classical ext) as [tn [cond [[tnLtT3 [m0 mrecvm0]] notAfter]]].
-      
-      pose proof (recvImpMarkSend mrecvm0) as [tr [trLeTn msendm0]].
-      assert (opts: tr = t1 \/ tr > t1 \/ tr < t1) by omega.
-      destruct opts as [trEqT1 | [trGtT1 | trLtT1]].
-      rewrite trEqT1 in *.
-      pose proof (uniqMarksend1 msendm msendm0) as mEqm0.
-      rewrite <- mEqm0 in *.
-      generalize neg cond mrecvm0; clear; firstorder.
-      assert (tnLeT: tn <= t) by omega.
-      assert (cond2: forall t4, t4 < tn -> ~ recv mch c p a t4 m) by (
-        intros t4 t4LtTn; assert (t4LtT3: t4 < t3) by omega;
-          generalize neg t4LtT3; clear; firstorder).
-      apply (cRespResp t1 tr tn tnLeT m msendm m0 msendm0 mrecvm0 trGtT1 cond2).
-      assert (notty2': ~ exists t'', tr <= t'' < t1 /\ exists m, recv mch p c a t'' m /\ to m >= state c a t1) by (
-        unfold not; intros [t'' [cond2 [m1 [mrecvm1 _]]]];
-          pose proof (recvImpMarkSend mrecvm1) as [t5 [t5LeT'' msendm1]];
-            assert (trLeT: tr <= t) by omega;
-              assert (t5LeT: t5 <= t) by omega;
-                assert (one: forall tc', tc' < tr -> ~ recv mch p c a tc' m1) by (
-                  unfold not; intros tc' tc'LtTr mrecv'm1;
-                    pose proof (uniqRecv2 mrecvm1 mrecv'm1) as t''EqTc';
-                      rewrite <- t''EqTc' in *;
-                        omega);
-                assert (two: forall tp', tp' < t5 -> ~ recv mch c p a tp' m0) by (
-                  unfold not; intros tp' tp'LtT5 mrecv'm0;
-                    pose proof (uniqRecv2 mrecvm0 mrecv'm0) as tnEqTp';
-                      rewrite <- tnEqTp' in *; omega);
-                apply (cross tr t5 trLeT t5LeT m0 msendm0 m1 msendm1 one two)).
-      assert (notty2: ~ exists t'', S tr <= t'' < t1 /\ exists m, recv mch p c a t'' m /\ to m >= state c a t1) by (
-        unfold not; intros [t'' [cond1 rest]]; assert (cond2: tr <= t'' < t1) by omega;
-          generalize notty2' cond2 rest; clear; firstorder).
-      assert (strLeT1: S tr <= t1) by omega.
-      pose proof (whenChildHighConv strLeT1 notty2) as st1LeTr.
-      pose proof (whenChildHighConv t1LtT2 notty) as sST1LeT2.
-      assert (trLtT3: tr < t3) by omega.
-      assert (noC: forall tn0, S tn <= tn0 < t3 -> (forall m, ~ marksend mch p c a tn0 m) /\
-        (forall m, ~ recv mch c p a tn0 m)) by (
+    destruct (classical (exists tn, tn < t3 /\ t1 <= tn /\ exists m0, recv mch c p a tn m0)) as [ext|noEx].
+    pose proof (maxExists' classical ext) as [tn [cond [[tnLtT3 [m0 mrecvm0]] notAfter]]].
+    
+    pose proof (recvImpMarkSend mrecvm0) as [tr [trLeTn msendm0]].
+    assert (opts: tr = t1 \/ tr > t1 \/ tr < t1) by omega.
+    destruct opts as [trEqT1 | [trGtT1 | trLtT1]].
+    rewrite trEqT1 in *.
+    pose proof (uniqMarksend1 msendm msendm0) as mEqm0.
+    rewrite <- mEqm0 in *.
+    generalize neg cond mrecvm0; clear; firstorder.
+    assert (tnLeT: tn <= t) by omega.
+    assert (cond2: forall t4, t4 < tn -> ~ recv mch c p a t4 m) by (
+      intros t4 t4LtTn; assert (t4LtT3: t4 < t3) by omega;
+        generalize neg t4LtT3; clear; firstorder).
+    apply (cRespResp t1 tr tn tnLeT m msendm m0 msendm0 mrecvm0 trGtT1 cond2).
+    assert (notty2': ~ exists t'', tr <= t'' < t1 /\ exists m, recv mch p c a t'' m /\ to m >= state c a t1) by (
+      unfold not; intros [t'' [cond2 [m1 [mrecvm1 _]]]];
+        pose proof (recvImpMarkSend mrecvm1) as [t5 [t5LeT'' msendm1]];
+          assert (trLeT: tr <= t) by omega;
+            assert (t5LeT: t5 <= t) by omega;
+              assert (one: forall tc', tc' < tr -> ~ recv mch p c a tc' m1) by (
+                unfold not; intros tc' tc'LtTr mrecv'm1;
+                  pose proof (uniqRecv2 mrecvm1 mrecv'm1) as t''EqTc';
+                    rewrite <- t''EqTc' in *;
+                      omega);
+              assert (two: forall tp', tp' < t5 -> ~ recv mch c p a tp' m0) by (
+                unfold not; intros tp' tp'LtT5 mrecv'm0;
+                  pose proof (uniqRecv2 mrecvm0 mrecv'm0) as tnEqTp';
+                    rewrite <- tnEqTp' in *; omega);
+              apply (cross tr t5 trLeT t5LeT m0 msendm0 m1 msendm1 one two)).
+    assert (notty2: ~ exists t'', S tr <= t'' < t1 /\ exists m, recv mch p c a t'' m /\ to m >= state c a t1) by (
+      unfold not; intros [t'' [cond1 rest]]; assert (cond2: tr <= t'' < t1) by omega;
+        generalize notty2' cond2 rest; clear; firstorder).
+    assert (strLeT1: S tr <= t1) by omega.
+    pose proof (st.whenChildHighConv strLeT1 notty2) as st1LeTr.
+    pose proof (st.whenChildHighConv t1LtT2 notty) as sST1LeT2.
+    assert (trLtT3: tr < t3) by omega.
+    assert (noC: forall tn0, S tn <= tn0 < t3 -> (forall m, ~ marksend mch p c a tn0 m) /\
+      (forall m, ~ recv mch c p a tn0 m)) by (
         intros tn0 cond2;
           constructor; [assert (cond3: t1 <= tn0 < t3) by omega; generalize noSend cond3; clear; firstorder|
             assert (cond4: tn < tn0 < t3) by omega; 
               assert (t1LeTn0: t1 <= tn0) by omega; generalize cond4 t1LeTn0 notAfter; clear; firstorder]).
-      assert (sTnLtT3: S tn <= t3) by omega.
-      pose proof (db.noChange2 sTnLtT3 noC) as dirEq.
-      unfold Dir.st in *.
-      generalize st1LeTr sST1LeT2 sTnLtT3 dirEq rsendr rrecvr msendm msendm0 mrecvm0; clear; intros.
-      pose proof (sb.sendmChange msendm) as sEqTom.
-      pose proof (stSendmImpSt msendm) as sGtTom.
-      pose proof (db.recvmChange mrecvm0) as dSEqTom0.
-      pose proof (sb.sendmChange msendm0) as sSEqTom0.
-      pose proof (dirRecvmCond rrecvr) as dLeFromr.
-      pose proof (sb.sendmFrom rsendr) as sEqFromr.
-      unfold St.st, Dir.st in *. omega.
-      generalize sendRecv noSend noEx; clear; firstorder.
-    Qed.
+    assert (sTnLtT3: S tn <= t3) by omega.
+    pose proof (dir.noChange2 sTnLtT3 noC) as dirEq.
+    unfold dir.st in *.
+    generalize st1LeTr sST1LeT2 sTnLtT3 dirEq rsendr rrecvr msendm msendm0 mrecvm0; clear; intros.
+    pose proof (st.sendmChange msendm) as sEqTom.
+    pose proof (st.sendmImpSt msendm) as sGtTom.
+    pose proof (dir.recvmChange mrecvm0) as dSEqTom0.
+    pose proof (st.sendmChange msendm0) as sSEqTom0.
+    pose proof (dir.recvmCond rrecvr) as dLeFromr.
+    pose proof (st.sendmFrom rsendr) as sEqFromr.
+    unfold st.st, dir.st in *. omega.
+    generalize sendRecv noSend noEx; clear; firstorder.
+  Qed.
 
-    Theorem conservative: forall {a t}, dir p c a t >= state c a t.
-    Proof.
-      intros a t.
-      pose proof (@mainInd a t) as [first _].
-      assert (tLeT: t <= t) by omega; firstorder.
-    Qed.
+  Theorem conservative: forall {a t}, dir p c a t >= state c a t.
+  Proof.
+    intros a t.
+    pose proof (@mainInd a t) as [first _].
+    assert (tLeT: t <= t) by omega; firstorder.
+  Qed.
 
-    Lemma cRespFifo: forall {a t1 t2 t3 m1 m2}, marksend mch c p a t1 m1 -> marksend mch c p a t2 m2 ->
-      recv mch c p a t3 m2 -> t1 < t2 -> (forall t4, t4 < t3 -> ~ recv mch c p a t4 m1) -> False.
-    Proof.
-      intros a t1 t2 t3 m1 m2 sendm1 sendm2 recvm2 t1LtT2.
-      pose proof (@mainInd a t3) as [_ [_ [_ last]]].
-      specialize (last t1 t2 t3).
-      assert (t3LeT3: t3 <= t3) by omega.
-      firstorder.
-    Qed.
+  Lemma cRespFifo: forall {a t1 t2 t3 m1 m2}, marksend mch c p a t1 m1 -> marksend mch c p a t2 m2 ->
+    recv mch c p a t3 m2 -> t1 < t2 -> (forall t4, t4 < t3 -> ~ recv mch c p a t4 m1) -> False.
+  Proof.
+    intros a t1 t2 t3 m1 m2 sendm1 sendm2 recvm2 t1LtT2.
+    pose proof (@mainInd a t3) as [_ [_ [_ last]]].
+    specialize (last t1 t2 t3).
+    assert (t3LeT3: t3 <= t3) by omega.
+    firstorder.
+  Qed.
 
-    Lemma cross: forall {a t1 t2 m1 m2}, marksend mch c p a t1 m1 -> marksend mch p c a t2 m2 ->
-      (forall t3, t3 < t1 -> ~ recv mch p c a t3 m2) -> (forall t4, t4 < t2 -> ~ recv mch c p a t4 m1) -> False.
-      intros a t1 t2 m1 m2 sendm1 sendm2 one two.
-      assert (opts: t1 <= t2 \/ t1 > t2) by omega.
-      destruct opts as [t1LeT2 | t2LtT1].
-      assert (t2LeT2: t2 <= t2) by omega.
-      pose proof (@mainInd a t2) as [_ [sec _]].
-      apply (sec t1 t2 t1LeT2 t2LeT2 m1 sendm1 m2 sendm2 one two).
-      assert (t2LeT1: t2 <= t1) by omega.
-      assert (t1LeT1: t1 <= t1) by omega.
-      pose proof (@mainInd a t1) as [_ [sec _]].
-      apply (sec t1 t2 t1LeT1 t2LeT1 m1 sendm1 m2 sendm2 one two).
-    Qed.
+  Lemma cross: forall {a t1 t2 m1 m2}, marksend mch c p a t1 m1 -> marksend mch p c a t2 m2 ->
+    (forall t3, t3 < t1 -> ~ recv mch p c a t3 m2) -> (forall t4, t4 < t2 -> ~ recv mch c p a t4 m1) -> False.
+    intros a t1 t2 m1 m2 sendm1 sendm2 one two.
+    assert (opts: t1 <= t2 \/ t1 > t2) by omega.
+    destruct opts as [t1LeT2 | t2LtT1].
+    assert (t2LeT2: t2 <= t2) by omega.
+    pose proof (@mainInd a t2) as [_ [sec _]].
+    apply (sec t1 t2 t1LeT2 t2LeT2 m1 sendm1 m2 sendm2 one two).
+    assert (t2LeT1: t2 <= t1) by omega.
+    assert (t1LeT1: t1 <= t1) by omega.
+    pose proof (@mainInd a t1) as [_ [sec _]].
+    apply (sec t1 t2 t1LeT1 t2LeT1 m1 sendm1 m2 sendm2 one two).
+  Qed.
 
-    Theorem cReqRespSent: forall {a t1 t2 r}, marksend rch p c a t1 r -> recv rch p c a t2 r ->
-      to r >= state c a t2 -> exists t3, t3 < t2 /\ exists m, marksend mch c p a t3 m /\ to m <= to r /\
-        (forall t4, t4 < t1 -> ~ recv mch c p a t4 m).
-    Proof.
-      intros a t1 t2 r sendr recvr toRGestT2.
-      destruct (classical (exists t3, t3 < t2 /\ exists m, marksend mch c p a t3 m /\ to m <= to r /\ forall t4,
-        t4 < t1 -> ~ recv mch c p a t4 m)) as [easy|hard].
-      intuition.
-      pose proof (recvImpMarkSend recvr) as [t1' [t1LeT2 send'r]].
-      pose proof (uniqMarksend2 sendr send'r) as t1'EqT1.
-      rewrite <- t1'EqT1 in *.
-      clear t1'EqT1 send'r t1'.
+  Theorem cReqRespSent: forall {a t1 t2 r}, marksend rch p c a t1 r -> recv rch p c a t2 r ->
+    to r >= state c a t2 -> exists t3, t3 < t2 /\ exists m, marksend mch c p a t3 m /\ to m <= to r /\
+      (forall t4, t4 < t1 -> ~ recv mch c p a t4 m).
+  Proof.
+    intros a t1 t2 r sendr recvr toRGestT2.
+    destruct (classical (exists t3, t3 < t2 /\ exists m, marksend mch c p a t3 m /\ to m <= to r /\ forall t4,
+      t4 < t1 -> ~ recv mch c p a t4 m)) as [easy|hard].
+    intuition.
+    pose proof (recvImpMarkSend recvr) as [t1' [t1LeT2 send'r]].
+    pose proof (uniqMarksend2 sendr send'r) as t1'EqT1.
+    rewrite <- t1'EqT1 in *.
+    clear t1'EqT1 send'r t1'.
 
-      destruct (classical (exists t, t < t1 /\ ((exists m, recv mch c p a t m) \/
-        (exists m, marksend mch p c a t m)))) as [ex | notEx].
-      pose proof (maxExists' classical ex) as [t [tLtT1 [sendOrRecv notAfter]]].
-      assert (nothing: forall y, S t <= y < t1 -> (forall m, ~ marksend mch p c a y m) /\
-        (forall m, ~ recv mch c p a y m)) by
-      (intros y cond; assert (cond2: t < y < t1)by omega; generalize cond2 notAfter; clear; firstorder).
-      pose proof (db.noChange2 tLtT1 nothing) as dirEq.
-      clear nothing; unfold Dir.st in *.
-      destruct sendOrRecv as [[m recvm] | [m sendm]].
-      pose proof (recvImpMarkSend recvm) as [t' [t'LeT sendm]].
-      assert (noCRecv: forall tm, t' <= tm < t2 -> forall m', ~ recv mch p c a tm m') by (
-        unfold not; intros tm cond m' recvm';
-          pose proof (recvImpMarkSend recvm') as [ts [tsLeTm sendm']];
-            assert (opts: ts < t \/ ts = t \/ t < ts < t1 \/ t1 <= ts) by omega;
-              destruct opts as [tsLtT | [tsEqT | [tLtTsLtT1  | t1LeTs ]]]; [
-                assert (one: forall x, x < t' -> ~ recv mch p c a x m') by ( unfold not; intros x xLtT' recv'm';
-                  pose proof (uniqRecv2 recvm' recv'm') as xEqTm; omega);
-                assert (two: forall x, x < ts -> ~ recv mch c p a x m) by (unfold not; intros x xLtTs recv'm;
-                  pose proof (uniqRecv2 recvm recv'm) as xEqTs; omega);
-                apply (cross sendm sendm' one two) |
-                  rewrite tsEqT in *;
-                    apply (db.noSendmRecvm sendm' recvm) |
-                      generalize notAfter tLtTsLtT1 sendm'; clear; firstorder |
-                        pose proof (pReqResp noTwoPResp noTwoPReqNon sendr sendm' recvm' t1LeTs) as [t4 [t4LtTm recv'r]];
-      pose proof (uniqRecv2 recvr recv'r) as t4EqT2; omega]).
-      destruct (classical (exists ts, ts < t2 /\ t' < ts /\ exists m', marksend mch c p a ts m'))
-        as [ ex2 | notEx2].
-      pose proof (maxExists' classical ex2) as [ts [tsLtT2 [[t'LtTs [m' sendm']] notAfter2]]].
-      assert (nothing: forall y, S ts <= y < t2 ->
-        (forall m, ~ marksend mch c p a y m) /\ (forall m, ~ recv mch p c a y m)) by
-      (intros y cond; assert (cond1: t' < y < t2) by omega; assert (cond2: t' <= y < t2) by omega;
-        generalize notAfter2 noCRecv cond cond1 cond2; clear; firstorder).
-      pose proof (sb.noChange2 tsLtT2 nothing) as stEq.
-      unfold St.st in *.
-      destruct (classical (exists tr, tr < t1 /\ recv mch c p a tr m')) as [ [tr [trLtT1 recvm']] | noRecv].
-      assert (opts: tr < t \/ tr = t \/ t < tr < t1) by omega.
-      destruct opts as [trLtT | [trEqT | cond]].
-      assert (forall t4, t4 < tr -> ~ recv mch c p a t4 m) by (
-        unfold not; intros t4 t4LtTr recv'm; pose proof (uniqRecv2 recvm recv'm) as t4EqT; omega).
-      pose proof (cRespFifo sendm sendm' recvm' t'LtTs). intuition.
-      rewrite trEqT in *.
-      pose proof (uniqRecv1 recvm recvm') as mEqM'.
-      rewrite mEqM' in *.
-      pose proof (uniqMarksend2 sendm sendm') as t'EqTs.
-      omega.
-      generalize notAfter cond recvm'; clear; firstorder.
-      assert (opts: to m' <= to r \/ to m' > to r) by omega.
-      destruct opts as [toM'LeToR | toM'GtToR].
-      generalize tsLtT2 sendm' toM'LeToR noRecv; clear; firstorder.
-      pose proof (sb.sendmChange sendm') as stEqToM'.
-      unfold St.st in *.
-      omega.
-      assert (nothing: forall y, S t' <= y < t2 ->
-        (forall m, ~ marksend mch c p a y m) /\ (forall m, ~ recv mch p c a y m)) by
-      (intros y cond; assert (cond2: t' <= y < t2) by omega;
-        generalize notEx2 noCRecv cond cond2; clear; firstorder).
-      assert (t'LeT2: S t' <= t2) by omega.
-      pose proof (sb.noChange2 t'LeT2 nothing) as stEq.
-      pose proof (db.sendrImpSt sendr) as toRLtD.
-      pose proof (sb.sendmChange sendm) as st1.
-      pose proof (db.recvmChange recvm) as st2.
-      unfold St.st, Dir.st, Dir.toRSComp in *.
-      omega.
+    destruct (classical (exists t, t < t1 /\ ((exists m, recv mch c p a t m) \/
+      (exists m, marksend mch p c a t m)))) as [ex | notEx].
+    pose proof (maxExists' classical ex) as [t [tLtT1 [sendOrRecv notAfter]]].
+    assert (nothing: forall y, S t <= y < t1 -> (forall m, ~ marksend mch p c a y m) /\
+      (forall m, ~ recv mch c p a y m)) by
+    (intros y cond; assert (cond2: t < y < t1)by omega; generalize cond2 notAfter; clear; firstorder).
+    pose proof (dir.noChange2 tLtT1 nothing) as dirEq.
+    clear nothing; unfold dir.st in *.
+    destruct sendOrRecv as [[m recvm] | [m sendm]].
+    pose proof (recvImpMarkSend recvm) as [t' [t'LeT sendm]].
+    assert (noCRecv: forall tm, t' <= tm < t2 -> forall m', ~ recv mch p c a tm m') by (
+      unfold not; intros tm cond m' recvm';
+        pose proof (recvImpMarkSend recvm') as [ts [tsLeTm sendm']];
+          assert (opts: ts < t \/ ts = t \/ t < ts < t1 \/ t1 <= ts) by omega;
+            destruct opts as [tsLtT | [tsEqT | [tLtTsLtT1  | t1LeTs ]]]; [
+              assert (one: forall x, x < t' -> ~ recv mch p c a x m') by ( unfold not; intros x xLtT' recv'm';
+                pose proof (uniqRecv2 recvm' recv'm') as xEqTm; omega);
+              assert (two: forall x, x < ts -> ~ recv mch c p a x m) by (unfold not; intros x xLtTs recv'm;
+                pose proof (uniqRecv2 recvm recv'm) as xEqTs; omega);
+              apply (cross sendm sendm' one two) |
+                rewrite tsEqT in *;
+                  apply (dir.noSendmRecvm sendm' recvm) |
+                    generalize notAfter tLtTsLtT1 sendm'; clear; firstorder |
+                      pose proof (pReqResp noTwoPResp noTwoPReqNon sendr sendm' recvm' t1LeTs) as [t4 [t4LtTm recv'r]];
+                        pose proof (uniqRecv2 recvr recv'r) as t4EqT2; omega]).
+    destruct (classical (exists ts, ts < t2 /\ t' < ts /\ exists m', marksend mch c p a ts m'))
+      as [ ex2 | notEx2].
+    pose proof (maxExists' classical ex2) as [ts [tsLtT2 [[t'LtTs [m' sendm']] notAfter2]]].
+    assert (nothing: forall y, S ts <= y < t2 ->
+      (forall m, ~ marksend mch c p a y m) /\ (forall m, ~ recv mch p c a y m)) by
+    (intros y cond; assert (cond1: t' < y < t2) by omega; assert (cond2: t' <= y < t2) by omega;
+      generalize notAfter2 noCRecv cond cond1 cond2; clear; firstorder).
+    pose proof (st.noChange2 tsLtT2 nothing) as stEq.
+    unfold st.st in *.
+    destruct (classical (exists tr, tr < t1 /\ recv mch c p a tr m')) as [ [tr [trLtT1 recvm']] | noRecv].
+    assert (opts: tr < t \/ tr = t \/ t < tr < t1) by omega.
+    destruct opts as [trLtT | [trEqT | cond]].
+    assert (forall t4, t4 < tr -> ~ recv mch c p a t4 m) by (
+      unfold not; intros t4 t4LtTr recv'm; pose proof (uniqRecv2 recvm recv'm) as t4EqT; omega).
+    pose proof (cRespFifo sendm sendm' recvm' t'LtTs). intuition.
+    rewrite trEqT in *.
+    pose proof (uniqRecv1 recvm recvm') as mEqM'.
+    rewrite mEqM' in *.
+    pose proof (uniqMarksend2 sendm sendm') as t'EqTs.
+    omega.
+    generalize notAfter cond recvm'; clear; firstorder.
+    assert (opts: to m' <= to r \/ to m' > to r) by omega.
+    destruct opts as [toM'LeToR | toM'GtToR].
+    generalize tsLtT2 sendm' toM'LeToR noRecv; clear; firstorder.
+    pose proof (st.sendmChange sendm') as stEqToM'.
+    unfold st.st in *.
+    omega.
+    assert (nothing: forall y, S t' <= y < t2 ->
+      (forall m, ~ marksend mch c p a y m) /\ (forall m, ~ recv mch p c a y m)) by
+    (intros y cond; assert (cond2: t' <= y < t2) by omega;
+      generalize notEx2 noCRecv cond cond2; clear; firstorder).
+    assert (t'LeT2: S t' <= t2) by omega.
+    pose proof (st.noChange2 t'LeT2 nothing) as stEq.
+    pose proof (dir.sendrImpSt sendr) as toRLtD.
+    pose proof (st.sendmChange sendm) as st1.
+    pose proof (dir.recvmChange recvm) as st2.
+    unfold st.st, dir.st, dir.toRSComp in *.
+    omega.
 
-      assert (tLeT1: t <= t1) by omega.
-      pose proof (pRespReq noTwoPResp noTwoPReqNon sendm sendr recvr tLeT1) as [t' [t'LtT2 recvm]].
-      pose proof (recvImpMarkSend recvm) as [t'' [tLeT' send'm]].
-      pose proof (uniqMarksend2 sendm send'm) as t''EqT.
-      rewrite <- t''EqT in *. clear t''EqT t'' send'm.
-      assert (noCRecv: forall tm, t' < tm < t2 -> forall m', ~ recv mch p c a tm m').
-        unfold not; intros tm cond m' recvm';
-          pose proof (recvImpMarkSend recvm') as [ts [tsLeTm sendm']];
-            assert (opts: ts < t \/ ts = t \/ t < ts < t1 \/ t1 <= ts) by omega;
-              destruct opts as [tsLtT | [tsEqT | [tLtTsLtT1  | t1LeTs ]]]; [
-                pose proof (dirSendmImpRecvr sendm) as [r' recvr'];
-                  pose proof (recvImpMarkSend recvr') as [tx [txLeT sendr']];
-                    assert (one: forall t3, t3 < tx -> ~ recv mch p c a t3 m') by (
-                      unfold not; intros t3 t3LtTx recv'm'; pose proof (uniqRecv2 recvm' recv'm') as t3EqTr;
-                        omega);
-                    assert (two: forall t4, t4 <= ts -> ~ recv rch c p a t4 r') by (
-                      unfold not; intros t4 t4LeTs recv'r'; pose proof (uniqRecv2 recvr' recv'r') as t4EqTs;
-                        omega);
-                    apply (cReqPRespCross sendr' sendm' one two)|
+    assert (tLeT1: t <= t1) by omega.
+    pose proof (pRespReq noTwoPResp noTwoPReqNon sendm sendr recvr tLeT1) as [t' [t'LtT2 recvm]].
+    pose proof (recvImpMarkSend recvm) as [t'' [tLeT' send'm]].
+    pose proof (uniqMarksend2 sendm send'm) as t''EqT.
+    rewrite <- t''EqT in *. clear t''EqT t'' send'm.
+    assert (noCRecv: forall tm, t' < tm < t2 -> forall m', ~ recv mch p c a tm m').
+    unfold not; intros tm cond m' recvm';
+      pose proof (recvImpMarkSend recvm') as [ts [tsLeTm sendm']];
+        assert (opts: ts < t \/ ts = t \/ t < ts < t1 \/ t1 <= ts) by omega;
+          destruct opts as [tsLtT | [tsEqT | [tLtTsLtT1  | t1LeTs ]]]; [
+            pose proof (dir.sendmImpRecvr sendm) as [r' recvr'];
+              pose proof (recvImpMarkSend recvr') as [tx [txLeT sendr']];
+                assert (one: forall t3, t3 < tx -> ~ recv mch p c a t3 m') by (
+                  unfold not; intros t3 t3LtTx recv'm'; pose proof (uniqRecv2 recvm' recv'm') as t3EqTr;
+                    omega);
+                assert (two: forall t4, t4 <= ts -> ~ recv rch c p a t4 r') by (
+                  unfold not; intros t4 t4LeTs recv'r'; pose proof (uniqRecv2 recvr' recv'r') as t4EqTs;
+                    omega);
+                apply (cReqPRespCross sendr' sendm' one two)|
                   rewrite tsEqT in *; pose proof (uniqMarksend1 sendm sendm') as mEqM'; rewrite mEqM' in *;
                     pose proof (uniqRecv2 recvm recvm') as trEqT'; omega |
                       generalize notAfter tLtTsLtT1 sendm'; clear; firstorder |
                         pose proof (pReqResp noTwoPResp noTwoPReqNon sendr sendm' recvm' t1LeTs) as [t4 [t4LtTm recv'r]];
                           pose proof (uniqRecv2 recvr recv'r) as t4EqT2; omega].
-      
-      destruct (classical (exists ts, ts < t2 /\ t' < ts /\ exists m', marksend mch c p a ts m'))
-        as [ ex2 | notEx2].
-      pose proof (maxExists' classical ex2) as [ts [tsLtT2 [[t'LtTs [m' sendm']] notAfter2]]].
-      assert (nothing: forall y, S ts <= y < t2 ->
-        (forall m, ~ marksend mch c p a y m) /\ (forall m, ~ recv mch p c a y m)) by
-      (intros y cond; assert (cond1: t' < y < t2) by omega;
-        generalize notAfter2 noCRecv cond cond1; clear; firstorder).
-      pose proof (sb.noChange2 tsLtT2 nothing) as stEq.
-      unfold St.st in *.
-      destruct (classical (exists tr, tr < t1 /\ recv mch c p a tr m')) as [ [tr [trLtT1 recvm']] | noRecv].
-      pose proof (recvImpMarkSend recvm') as [ts' [ts'LeTr send'm']].
-      pose proof (uniqMarksend2 send'm' sendm') as ts'EqTs.
-      assert (trGtT: tr > t) by omega.
-      clear ts' ts'LeTr send'm' ts'EqTs.
-      assert (opts: t < tr < t1 \/ t1 <= tr) by omega.
-      destruct opts as [cond1 | t1LeTr].
-      generalize cond1 notAfter recvm'; clear; firstorder.
-      assert (opts: to m' <= to r \/ to m' > to r) by omega.
-      destruct opts as [toM'LeToR | toM'GtToR].
-      assert (noRecv: forall t4, t4 < t1 -> ~ recv mch c p a t4 m') by (
-        unfold not; intros t4 t4LtT1 recv'm'; pose proof (uniqRecv2 recvm' recv'm') as t4EqTr; omega).
-      generalize tsLtT2 sendm' toM'LeToR noRecv; clear; firstorder.
-      pose proof (sb.sendmChange sendm') as stEqToM'.
-      unfold St.st in *.
-      omega.
-      assert (last: forall t4, t4 < t1 -> ~ recv mch c p a t4 m') by (generalize noRecv; clear; firstorder).
-      assert (opts: to m' <= to r \/ to m' > to r) by omega.
-      destruct opts as [toM'LeToR | toM'GtToR].
-      generalize last tsLtT2 toM'LeToR sendm'; clear; firstorder.
-      pose proof (sb.sendmChange sendm') as stEqToM'.
-      unfold St.st in *.
-      omega.
-      assert (nothing: forall y, S t' <= y < t2 ->
-        (forall m, ~ marksend mch c p a y m) /\ (forall m, ~ recv mch p c a y m)) by
-      (generalize noCRecv notEx2; clear; firstorder).
-      pose proof (sb.noChange2 t'LtT2 nothing) as stEq.
-      unfold St.st in *.
-      pose proof (sb.recvmChange recvm) as st1.
-      pose proof (db.sendmChange sendm) as d1.
-      pose proof (db.sendrImpSt sendr) as d2.
-      unfold Dir.toRSComp, Dir.st, St.st in *.
-      omega.
-      assert (cNoRecv: forall t4, t4 < t2 -> forall m, ~ recv mch p c a t4 m) by (
-        unfold not; intros t4 t4LtT2 m recvm; pose proof (recvImpMarkSend recvm) as [t3 [t3LeT4 sendm]];
-          assert (opts: t3 < t1 \/ t3 >= t1) by omega;
-            destruct opts as [t3LtT1 | t4GeT1]; [
-              generalize notEx t3LtT1 sendm; clear; firstorder;
-                intuition |
-                  pose proof (pReqResp noTwoPResp noTwoPReqNon sendr sendm recvm t4GeT1) as [t5 [t4LtT4 recv'r]];
-                    pose proof (uniqRecv2 recvr recv'r) as t5EqT2; omega]).
-      destruct (classical (exists t3, t3 < t2 /\ exists m, marksend mch c p a t3 m)) as [ex2 | notEx2].
-      pose proof (maxExists' classical ex2) as [ts [tsLtT2 [[m' sendm'] notAfter2]]].
-      assert (nothing: forall y, S ts <= y < t2 ->
-        (forall m, ~ marksend mch c p a y m) /\ (forall m, ~ recv mch p c a y m)) by
-      (intros y cond;
-        generalize notAfter2 cNoRecv cond; clear; firstorder).
-      pose proof (sb.noChange2 tsLtT2 nothing) as stEq.
-      unfold St.st in *.
-      destruct (classical (exists tr, tr < t1 /\ recv mch c p a tr m')) as [ [tr [trLtT1 recvm']] | noRecv].
-      generalize notEx trLtT1 recvm'; clear; firstorder.
-      assert (opts: to m' <= to r \/ to m' > to r) by omega.
-      destruct opts as [toM'LeToR | toM'GtToR].
-      generalize toM'LeToR noRecv tsLtT2 sendm'; clear; firstorder.
-      pose proof (sb.sendmChange sendm') as stEqToM'.
-      unfold St.st in *.
-      omega.
-      assert (nothing1: forall y, 0 <= y < t2 ->
-        (forall m, ~ marksend mch c p a y m) /\ (forall m, ~ recv mch p c a y m)) by
-      (generalize cNoRecv notEx2; clear; firstorder).
-      assert (x1: 0 <= t2) by omega.
-      pose proof (sb.noChange2 x1 nothing1) as st1.
-      assert (nothing2: forall y, 0 <= y < t1 ->
-        (forall m, ~ marksend mch p c a y m) /\ (forall m, ~ recv mch c p a y m)) by
-      (generalize notEx; clear; firstorder).
-      assert (x2: 0 <= t1) by omega.
-      pose proof (db.noChange2 x2 nothing2) as d1.
-      pose proof (init a) as start.
-      pose proof (db.sendrImpSt sendr) as d2.
-      unfold Dir.toRSComp, Dir.st, St.st in *.
-      omega.
-    Qed.
-  End LocalRules.
-End System.
-
+    
+    destruct (classical (exists ts, ts < t2 /\ t' < ts /\ exists m', marksend mch c p a ts m'))
+      as [ ex2 | notEx2].
+    pose proof (maxExists' classical ex2) as [ts [tsLtT2 [[t'LtTs [m' sendm']] notAfter2]]].
+    assert (nothing: forall y, S ts <= y < t2 ->
+      (forall m, ~ marksend mch c p a y m) /\ (forall m, ~ recv mch p c a y m)) by
+    (intros y cond; assert (cond1: t' < y < t2) by omega;
+      generalize notAfter2 noCRecv cond cond1; clear; firstorder).
+    pose proof (st.noChange2 tsLtT2 nothing) as stEq.
+    unfold st.st in *.
+    destruct (classical (exists tr, tr < t1 /\ recv mch c p a tr m')) as [ [tr [trLtT1 recvm']] | noRecv].
+    pose proof (recvImpMarkSend recvm') as [ts' [ts'LeTr send'm']].
+    pose proof (uniqMarksend2 send'm' sendm') as ts'EqTs.
+    assert (trGtT: tr > t) by omega.
+    clear ts' ts'LeTr send'm' ts'EqTs.
+    assert (opts: t < tr < t1 \/ t1 <= tr) by omega.
+    destruct opts as [cond1 | t1LeTr].
+    generalize cond1 notAfter recvm'; clear; firstorder.
+    assert (opts: to m' <= to r \/ to m' > to r) by omega.
+    destruct opts as [toM'LeToR | toM'GtToR].
+    assert (noRecv: forall t4, t4 < t1 -> ~ recv mch c p a t4 m') by (
+      unfold not; intros t4 t4LtT1 recv'm'; pose proof (uniqRecv2 recvm' recv'm') as t4EqTr; omega).
+    generalize tsLtT2 sendm' toM'LeToR noRecv; clear; firstorder.
+    pose proof (st.sendmChange sendm') as stEqToM'.
+    unfold st.st in *.
+    omega.
+    assert (last: forall t4, t4 < t1 -> ~ recv mch c p a t4 m') by (generalize noRecv; clear; firstorder).
+    assert (opts: to m' <= to r \/ to m' > to r) by omega.
+    destruct opts as [toM'LeToR | toM'GtToR].
+    generalize last tsLtT2 toM'LeToR sendm'; clear; firstorder.
+    pose proof (st.sendmChange sendm') as stEqToM'.
+    unfold st.st in *.
+    omega.
+    assert (nothing: forall y, S t' <= y < t2 ->
+      (forall m, ~ marksend mch c p a y m) /\ (forall m, ~ recv mch p c a y m)) by
+    (generalize noCRecv notEx2; clear; firstorder).
+    pose proof (st.noChange2 t'LtT2 nothing) as stEq.
+    unfold st.st in *.
+    pose proof (st.recvmChange recvm) as st1.
+    pose proof (dir.sendmChange sendm) as d1.
+    pose proof (dir.sendrImpSt sendr) as d2.
+    unfold dir.toRSComp, dir.st, st.st in *.
+    omega.
+    assert (cNoRecv: forall t4, t4 < t2 -> forall m, ~ recv mch p c a t4 m) by (
+      unfold not; intros t4 t4LtT2 m recvm; pose proof (recvImpMarkSend recvm) as [t3 [t3LeT4 sendm]];
+        assert (opts: t3 < t1 \/ t3 >= t1) by omega;
+          destruct opts as [t3LtT1 | t4GeT1]; [
+            generalize notEx t3LtT1 sendm; clear; firstorder;
+              intuition |
+                pose proof (pReqResp noTwoPResp noTwoPReqNon sendr sendm recvm t4GeT1) as [t5 [t4LtT4 recv'r]];
+                  pose proof (uniqRecv2 recvr recv'r) as t5EqT2; omega]).
+    destruct (classical (exists t3, t3 < t2 /\ exists m, marksend mch c p a t3 m)) as [ex2 | notEx2].
+    pose proof (maxExists' classical ex2) as [ts [tsLtT2 [[m' sendm'] notAfter2]]].
+    assert (nothing: forall y, S ts <= y < t2 ->
+      (forall m, ~ marksend mch c p a y m) /\ (forall m, ~ recv mch p c a y m)) by
+    (intros y cond;
+      generalize notAfter2 cNoRecv cond; clear; firstorder).
+    pose proof (st.noChange2 tsLtT2 nothing) as stEq.
+    unfold st.st in *.
+    destruct (classical (exists tr, tr < t1 /\ recv mch c p a tr m')) as [ [tr [trLtT1 recvm']] | noRecv].
+    generalize notEx trLtT1 recvm'; clear; firstorder.
+    assert (opts: to m' <= to r \/ to m' > to r) by omega.
+    destruct opts as [toM'LeToR | toM'GtToR].
+    generalize toM'LeToR noRecv tsLtT2 sendm'; clear; firstorder.
+    pose proof (st.sendmChange sendm') as stEqToM'.
+    unfold st.st in *.
+    omega.
+    assert (nothing1: forall y, 0 <= y < t2 ->
+      (forall m, ~ marksend mch c p a y m) /\ (forall m, ~ recv mch p c a y m)) by
+    (generalize cNoRecv notEx2; clear; firstorder).
+    assert (x1: 0 <= t2) by omega.
+    pose proof (st.noChange2 x1 nothing1) as st1.
+    assert (nothing2: forall y, 0 <= y < t1 ->
+      (forall m, ~ marksend mch p c a y m) /\ (forall m, ~ recv mch c p a y m)) by
+    (generalize notEx; clear; firstorder).
+    assert (x2: 0 <= t1) by omega.
+    pose proof (dir.noChange2 x2 nothing2) as d1.
+    pose proof (@init a) as start.
+    pose proof (dir.sendrImpSt sendr) as d2.
+    unfold dir.toRSComp, dir.st, dir.st, stSemi.st in *.
+    omega.
+  Qed.
+End PairTheorems.
